examples/mc-logic/arm_instScript.sml
@@ -45,7 +45,7 @@ val ARM_PROG_type =
 val ARM_PROG2_type =
   ``:condition ->
      ('a ARMset -> bool) ->
-     word32 list ->
+     word32 list -> (word32 list # (word30 -> word30) -> bool) ->
      ('a ARMset -> bool) ->
     (('a ARMset -> bool) # 
       (word30 -> word30) -> bool) -> bool``;
@@ -279,8 +279,8 @@ val heap_list_SPLIT = prove(
   \\ ASM_SIMP_TAC bool_ss [list_read_update]);
 
 val ARM_PROG_INTRO_SEQ_RD = prove(
-  ``(!y. ARM_PROG2 c (P * M (addr30 x) y) code (Q y * M (addr30 x) y) {}) ==>
-    ARM_PROG2 c (P * heap d f * cond (x IN d /\ aligned x)) code  
+  ``(!y. ARM_PROG2 c (P * M (addr30 x) y) code C (Q y * M (addr30 x) y) {}) ==>
+    ARM_PROG2 c (P * heap d f * cond (x IN d /\ aligned x)) code C
                 (Q (f x) * heap d f) {}``,
   REWRITE_TAC [ARM_PROG_MOVE_COND,ARM_PROG2_def] 
   \\ ONCE_REWRITE_TAC [CONJ_COMM] \\ REPEAT STRIP_TAC THEN1 METIS_TAC []
@@ -288,8 +288,8 @@ val ARM_PROG_INTRO_SEQ_RD = prove(
   \\ METIS_TAC [ARM_PROG_FRAME,setSTAR_CLAUSES]);    
 
 val ARM_PROG_INTRO_SEQ_RD_WR = prove(
-  ``(!y. ARM_PROG2 c (P * M (addr30 x) y) code (Q y * M (addr30 x) q) {}) ==>
-    ARM_PROG2 c (P * heap d f * cond (x IN d /\ aligned x)) code  
+  ``(!y. ARM_PROG2 c (P * M (addr30 x) y) code C (Q y * M (addr30 x) q) {}) ==>
+    ARM_PROG2 c (P * heap d f * cond (x IN d /\ aligned x)) code C 
                 (Q (f x) * heap d (update x q f)) {}``,
   REWRITE_TAC [ARM_PROG_MOVE_COND,ARM_PROG2_def] 
   \\ ONCE_REWRITE_TAC [CONJ_COMM] \\ REPEAT STRIP_TAC THEN1 METIS_TAC []
@@ -301,8 +301,8 @@ val ARM_PROG_INTRO_SEQ_WR =
 
 val ARM_PROG_INTRO_SEQ_LIST_WR = prove(
   ``(!ys. (LENGTH ys = LENGTH qs) ==> 
-          ARM_PROG2 c (P * ms (addr30 x) ys) [code] (Q * ms (addr30 x) qs) {}) ==>
-    ARM_PROG2 c (P * heap d f * cond (seq_addresses x qs SUBSET d /\ aligned x /\ LENGTH qs <= 16)) [code]  
+          ARM_PROG2 c (P * ms (addr30 x) ys) [code] C (Q * ms (addr30 x) qs) {}) ==>
+    ARM_PROG2 c (P * heap d f * cond (seq_addresses x qs SUBSET d /\ aligned x /\ LENGTH qs <= 16)) [code] C 
                 (Q * heap d (list_update x qs f)) {}``,
   REWRITE_TAC [ARM_PROG_MOVE_COND,ARM_PROG2_def] 
   \\ ONCE_REWRITE_TAC [CONJ_COMM] \\ REPEAT STRIP_TAC THEN1 METIS_TAC []
@@ -313,8 +313,8 @@ val ARM_PROG_INTRO_SEQ_LIST_WR = prove(
 
 val ARM_PROG_INTRO_SEQ_LIST_RD = prove(
   ``(!ys. (LENGTH ys = LENGTH (qs:word32 list)) ==> 
-          ARM_PROG2 c (P * ms (addr30 x) ys) [code] (Q ys * ms (addr30 x) ys) {}) ==>
-    ARM_PROG2 c (P * heap d f * cond (seq_addresses x qs SUBSET d /\ aligned x /\ LENGTH qs <= 16)) [code]
+          ARM_PROG2 c (P * ms (addr30 x) ys) [code] C (Q ys * ms (addr30 x) ys) {}) ==>
+    ARM_PROG2 c (P * heap d f * cond (seq_addresses x qs SUBSET d /\ aligned x /\ LENGTH qs <= 16)) [code] C
                 (Q (list_read x qs f) * heap d f) {}``,
   REWRITE_TAC [ARM_PROG_MOVE_COND,ARM_PROG2_def] 
   \\ ONCE_REWRITE_TAC [CONJ_COMM] \\ REPEAT STRIP_TAC THEN1 METIS_TAC []
@@ -365,492 +365,6 @@ val FORALL_IN_ms_address_set = prove(
   \\ ASM_REWRITE_TAC [LE_MULT_LCANCEL]
   \\ ASSUME_TAC (INST_TYPE [``:'a``|->``:32``] w2n_lt)
   \\ FULL_SIMP_TAC (std_ss++SIZES_ss) []);
-
-
-
-(*
-(* ----------------------------------------------------------------------------- *)
-(* Lemmas for seq of M assertions                                                *)
-(* ----------------------------------------------------------------------------- *)
-
-val seq_def = Define `
-  (seq a [] = emp) /\
-  (seq a (x::xs) = M (addr30 a) x * seq (a+4w) xs)`;
-
-val seq_addresses_def = Define `
-  (seq_addresses (a:word32) [] = {}) /\ 
-  (seq_addresses a (x::xs) = a INSERT seq_addresses (a+4w) xs)`;
-
-val REPLACE_def = Define `
-  (REPLACE 0 x [] = []) /\
-  (REPLACE 0 x (y::ys) = x::ys) /\
-  (REPLACE (SUC n) x [] = []) /\
-  (REPLACE (SUC n) x (y::ys) = y::REPLACE n x ys)`;
-
-val WR_def = Define `WR x y zs = REPLACE (w2n x DIV 4) y zs`;
-val RD_def = Define `RD x zs = EL (w2n x DIV 4) zs`;
-
-val list_WR_def = Define `
-  (list_WR x [] zs = zs) /\
-  (list_WR x (y::ys) zs = WR x y (list_WR (x+4w) ys zs))`;
-
-val list_RD_def = Define `
-  (list_RD x [] zs = []) /\
-  (list_RD x (y::ts) zs = RD x zs :: list_RD (x + 4w) ts zs)`;
-
-val IN_seq_addresses = prove(
-  ``!zs x z. x IN seq_addresses z zs ==>
-             ?ys y xs. (zs = ys ++ y::xs) /\ (4w * wLENGTH ys = x - z)``,
-  Induct \\ REWRITE_TAC [seq_addresses_def,NOT_IN_EMPTY,IN_INSERT]
-  \\ REPEAT STRIP_TAC \\ ASM_REWRITE_TAC [WORD_SUB_REFL] << [
-    Q.EXISTS_TAC `[]` \\ Q.EXISTS_TAC `h` \\ Q.EXISTS_TAC `zs`
-    \\ REWRITE_TAC [wLENGTH_def,LENGTH,WORD_MULT_CLAUSES,APPEND],
-    Q.PAT_ASSUM `!x.b` IMP_RES_TAC \\ ASM_REWRITE_TAC []
-    \\ Q.EXISTS_TAC `h::ys` \\ Q.EXISTS_TAC `y` \\ Q.EXISTS_TAC `xs`
-    \\ FULL_SIMP_TAC bool_ss [APPEND,wLENGTH_def,LENGTH,ADD1,GSYM word_add_n2w,WORD_MULT_CLAUSES]
-    \\ ONCE_REWRITE_TAC [WORD_ADD_COMM] \\ REWRITE_TAC [WORD_SUB_PLUS,WORD_SUB_ADD]])
-
-val FINITE_seq_addresses = prove(
-  ``!z zs. FINITE (seq_addresses z zs)``,  
-  REWRITE_TAC [FINITE_DEF] \\ REPEAT STRIP_TAC \\ Q.SPEC_TAC (`z`,`z`) \\ Induct_on `zs`
-  \\ ASM_SIMP_TAC bool_ss [seq_addresses_def]);
- 
-val CARD_seq_addresses = prove(
-  ``!xs:word32 list x. LENGTH xs < 2**30 ==> (CARD (seq_addresses x xs) = LENGTH xs)``,
-  Induct
-  \\ REWRITE_TAC [CARD_EMPTY,seq_addresses_def,LENGTH]
-  \\ REWRITE_TAC [MATCH_MP (CONJUNCT2 CARD_DEF) (SPEC_ALL FINITE_seq_addresses)]    
-  \\ REPEAT STRIP_TAC
-  \\ Cases_on `x IN seq_addresses (x + 4w) (xs:word32 list)` 
-  \\ ASM_REWRITE_TAC [ADD1,EQ_ADD_RCANCEL] << [
-    IMP_RES_TAC IN_seq_addresses
-    \\ FULL_SIMP_TAC bool_ss [WORD_SUB_PLUS,WORD_SUB_REFL]
-    \\ `4w:word32 * wLENGTH (ys:word32 list) + 4w = (0w - 4w) + 4w` by ASM_REWRITE_TAC [WORD_EQ_ADD_RCANCEL]
-    \\ FULL_SIMP_TAC bool_ss [WORD_SUB_ADD,LENGTH,LENGTH_APPEND]
-    \\ FULL_SIMP_TAC (std_ss++SIZES_ss) [word_mul_n2w,word_add_n2w,wLENGTH_def,n2w_11]    
-    \\ `LENGTH ys < 1073741824` by DECIDE_TAC 
-    \\ FULL_SIMP_TAC bool_ss [GSYM (EVAL ``1+1+1+1``)]
-    \\ FULL_SIMP_TAC bool_ss [RIGHT_ADD_DISTRIB]
-    \\ FULL_SIMP_TAC bool_ss [MULT_CLAUSES] 
-    \\ `(LENGTH ys + LENGTH ys + LENGTH ys + LENGTH ys +
-           (1 + 1 + 1 + 1)) < 4294967296` by DECIDE_TAC
-    \\ FULL_SIMP_TAC bool_ss [LESS_MOD] \\ `F` by DECIDE_TAC, 
-    Q.PAT_ASSUM `!x.b` MATCH_MP_TAC \\ DECIDE_TAC]);
-
-val seq_addresses_SUBSET_SHORTER = prove(
-  ``!qs:word32 list zs:word32 list. 
-      LENGTH qs < 2**30 ==> LENGTH zs < 2**30 ==>
-      seq_addresses x qs SUBSET seq_addresses z zs ==> 
-      LENGTH qs <= LENGTH zs``,
-  REPEAT STRIP_TAC
-  \\ IMP_RES_TAC ((MATCH_MP CARD_SUBSET (SPEC_ALL FINITE_seq_addresses)))
-  \\ IMP_RES_TAC CARD_seq_addresses \\ METIS_TAC []);
-
-val IN_seq_addresses_LEMMA = prove(
-  ``!zs x y z. x IN seq_addresses y (z::zs) ==> 
-               (x = y) \/ (x - 4w) IN seq_addresses y (z::zs)``,
-  Induct \\ ONCE_REWRITE_TAC [seq_addresses_def]
-  \\ REWRITE_TAC [IN_INSERT] THEN1 METIS_TAC [NOT_IN_EMPTY,seq_addresses_def]
-  \\ REPEAT STRIP_TAC \\ ASM_REWRITE_TAC []
-  \\ `(x = y + 4w) \/ x - 4w IN seq_addresses (y + 4w) (h::zs)` by METIS_TAC []
-  \\ ASM_REWRITE_TAC [WORD_ADD_SUB]);
-
-val SUBSET_seq_addresses_LEMMA2 = prove(
-  ``!z zs. LENGTH (zs:word32 list) < 2 ** 30 ==> ~(z - 4w IN seq_addresses z zs)``,
-  REPEAT STRIP_TAC \\ IMP_RES_TAC IN_seq_addresses
-  \\ `LENGTH ys < LENGTH zs` by (ASM_REWRITE_TAC [LENGTH,LENGTH_APPEND] \\ DECIDE_TAC)
-  \\ `z - 4w - z = 0w - 4w` by 
-    (REWRITE_TAC [GSYM WORD_SUB_PLUS] \\ ONCE_REWRITE_TAC [WORD_ADD_COMM]
-     \\ REWRITE_TAC [WORD_SUB_PLUS,WORD_SUB_REFL])
-  \\ FULL_SIMP_TAC bool_ss [wLENGTH_def,LENGTH_APPEND]  \\ Q.ABBREV_TAC `N = LENGTH ys`
-  \\ `n2w (4 * SUC N) = 0w:word32` by    
-     (ASM_REWRITE_TAC [ADD1,GSYM word_add_n2w,GSYM word_mul_n2w,WORD_MULT_CLAUSES,GSYM wLENGTH_def]
-     \\ REWRITE_TAC [WORD_SUB_LZERO,GSYM word_sub_def,WORD_SUB_REFL])
-  \\ FULL_SIMP_TAC (std_ss++SIZES_ss) [n2w_11]
-  \\ `4 * SUC N < 4 * 1073741824` by 
-   (REWRITE_TAC [LT_MULT_LCANCEL] \\ FULL_SIMP_TAC std_ss [LENGTH,LESS_MOD] \\ DECIDE_TAC)
-  \\ FULL_SIMP_TAC bool_ss [EVAL ``4 * 1073741824``,LESS_MOD]
-  \\ FULL_SIMP_TAC bool_ss [RW1 [MULT_COMM] MULT]
-  \\ DECIDE_TAC);
-
-val IN_seq_addresses2 = prove(
-  ``!zs z q. q IN seq_addresses z zs = ?k. (q = z + n2w (4 * k)) /\ k < LENGTH zs``,
-  Induct \\ REWRITE_TAC [seq_addresses_def,LENGTH,NOT_IN_EMPTY,DECIDE ``~(k < 0)``]        
-  \\ ASM_REWRITE_TAC [IN_INSERT] \\ REPEAT STRIP_TAC
-  \\ Cases_on `q = z` \\ ASM_REWRITE_TAC []
-  THEN1 (Q.EXISTS_TAC `0` \\ REWRITE_TAC [MULT_CLAUSES,DECIDE ``0 < SUC n``,WORD_ADD_0])
-  \\ EQ_TAC \\ REPEAT STRIP_TAC << [
-    Q.EXISTS_TAC `SUC k`
-    \\ ASM_REWRITE_TAC [ADD1,LT_ADD_RCANCEL,GSYM word_add_n2w,GSYM word_mul_n2w]
-    \\ REWRITE_TAC [WORD_MULT_CLAUSES,WORD_ADD_ASSOC], 
-    Cases_on `k`
-    \\ FULL_SIMP_TAC bool_ss [MULT_CLAUSES,WORD_ADD_0,ADD1,LT_ADD_RCANCEL]
-    \\ Q.EXISTS_TAC `n` \\ FULL_SIMP_TAC bool_ss 
-      [MULT_CLAUSES,WORD_ADD_0,ADD1,LT_ADD_RCANCEL,word_add_n2w,GSYM WORD_ADD_ASSOC]]);
-  
-val LENGTH_LESS_EQ_NOT_IN_seq_addresses = prove(
-  ``!z zs. LENGTH (zs:word32 list) < 2 ** 30 = ~(z - 4w IN seq_addresses z zs)``,
-  REPEAT STRIP_TAC \\ EQ_TAC \\ REWRITE_TAC [SUBSET_seq_addresses_LEMMA2]
-  \\ Cases_on `LENGTH (zs:word32 list) < 2**30` \\ ASM_REWRITE_TAC []
-  \\ FULL_SIMP_TAC bool_ss [DECIDE ``~(n < m) = m <= n:num``]  
-  \\ REWRITE_TAC [IN_seq_addresses2,WORD_EQ_SUB_RADD]
-  \\ Q.EXISTS_TAC `2**30-1`    
-  \\ REWRITE_TAC [word_add_n2w,GSYM WORD_ADD_ASSOC]
-  \\ `0 < 2**30` by EVAL_TAC
-  \\ ASM_SIMP_TAC bool_ss [DECIDE ``0 < n /\ n <= k ==> n - 1 < k``]
-  \\ ONCE_REWRITE_TAC [GSYM n2w_mod]
-  \\ SIMP_TAC (std_ss++SIZES_ss) [WORD_ADD_0]);
-
-val FORALL_IN_seq_addresses = prove(
-  ``!xs x. 2**30 <= LENGTH xs ==> !p. (x + addr32 p) IN seq_addresses x xs``,
-  REPEAT STRIP_TAC \\ REWRITE_TAC [IN_seq_addresses2]
-  \\ Q.SPEC_TAC (`p`,`p`) \\ Cases_word \\ Q.EXISTS_TAC `n` \\ REWRITE_TAC [addr32_n2w]
-  \\ MATCH_MP_TAC LESS_LESS_EQ_TRANS
-  \\ Q.EXISTS_TAC `2**30` \\ ASM_REWRITE_TAC [] \\ FULL_SIMP_TAC (std_ss++SIZES_ss) []);
-
-val SUBSET_seq_addresses_LEMMA = prove(
-  ``!zs:word32 list z qs:'a list x.
-                LENGTH qs < 2**30 ==>  
-                LENGTH zs < 2**30 ==> 
-                seq_addresses x qs SUBSET seq_addresses x zs ==>
-                (qs = []) \/ 
-                ?ts xs. (zs = ts ++ xs) /\ (LENGTH qs = LENGTH ts)``,
-  Induct_on `qs` \\ REWRITE_TAC [] \\ REPEAT STRIP_TAC \\ DISJ2_TAC
-  \\ Cases_on `zs`  THEN1 (FULL_SIMP_TAC bool_ss 
-    [seq_addresses_def,SUBSET_DEF,NOT_IN_EMPTY,IN_INSERT] \\ METIS_TAC [])
-  \\ `seq_addresses (x+4w) qs SUBSET seq_addresses (x+4w) t` by ALL_TAC << [
-    FULL_SIMP_TAC bool_ss [seq_addresses_def,SUBSET_DEF,IN_INSERT]   
-    \\ REPEAT STRIP_TAC
-    \\ `(x' = x) \/ x' IN seq_addresses (x + 4w) t` by METIS_TAC []
-    \\ IMP_RES_TAC IN_seq_addresses
-    \\ FULL_SIMP_TAC bool_ss [WORD_SUB_PLUS,WORD_SUB_REFL]
-    \\ `4w * wLENGTH ys = x - x - 4w` by METIS_TAC []
-    \\ FULL_SIMP_TAC bool_ss [WORD_SUB_PLUS,WORD_SUB_REFL]
-    \\ `4w:word32 * wLENGTH (ys:'a list) + 4w = (0w - 4w) + 4w` by ASM_REWRITE_TAC [WORD_EQ_ADD_RCANCEL]
-    \\ FULL_SIMP_TAC bool_ss [WORD_SUB_ADD,LENGTH,LENGTH_APPEND]
-    \\ FULL_SIMP_TAC (std_ss++SIZES_ss) [word_mul_n2w,word_add_n2w,wLENGTH_def,n2w_11]    
-    \\ `LENGTH ys < 1073741824` by DECIDE_TAC 
-    \\ FULL_SIMP_TAC bool_ss [GSYM (EVAL ``1+1+1+1``)]
-    \\ FULL_SIMP_TAC bool_ss [RIGHT_ADD_DISTRIB]
-    \\ FULL_SIMP_TAC bool_ss [MULT_CLAUSES] 
-    \\ `(LENGTH ys + LENGTH ys + LENGTH ys + LENGTH ys +
-           (1 + 1 + 1 + 1)) < 4294967296` by DECIDE_TAC
-    \\ FULL_SIMP_TAC bool_ss [LESS_MOD] \\ `F` by DECIDE_TAC,
-    FULL_SIMP_TAC bool_ss [LENGTH]
-    \\ `LENGTH qs < 2 ** 30 /\ LENGTH t < 2 ** 30` by DECIDE_TAC
-    \\ `(qs = []) \/ ?ts xs. (t = ts ++ xs) /\ (LENGTH qs = LENGTH ts)` by METIS_TAC []
-    \\ ASM_REWRITE_TAC []
-    THEN1 (Q.EXISTS_TAC `[h']` \\ Q.EXISTS_TAC `t` \\ REWRITE_TAC [LENGTH,APPEND])
-    \\ Q.EXISTS_TAC `h'::ts`    
-    \\ Q.EXISTS_TAC `xs`
-    \\ ASM_REWRITE_TAC [LENGTH,APPEND]]);
-
-val SUBSET_seq_addresses = prove(
-  ``!zs:word32 list z qs:'a list x.
-       seq_addresses x qs SUBSET seq_addresses z zs ==>
-       LENGTH qs < 2**30 ==> 
-       LENGTH zs < 2**30 ==> 
-       (qs = []) \/ 
-       ?ys ts xs. (zs = ys ++ ts ++ xs) /\ (4w * wLENGTH ys = x - z) /\
-                  (LENGTH qs = LENGTH ts)``,
-  Induct_on `zs` \\ REPEAT STRIP_TAC \\ Cases_on `qs` \\ ASM_REWRITE_TAC []    
-  THEN1 (FULL_SIMP_TAC bool_ss [seq_addresses_def,SUBSET_DEF,NOT_IN_EMPTY,IN_INSERT] \\ METIS_TAC [])
-  \\ Cases_on `x = z` \\ DISJ2_TAC << [
-    ASM_REWRITE_TAC [WORD_SUB_REFL] \\ Q.EXISTS_TAC `[]`
-    \\ REWRITE_TAC [wLENGTH_def,word_mul_n2w,MULT_CLAUSES,LENGTH,APPEND]
-    \\ MATCH_MP_TAC (RW [LENGTH,NOT_CONS_NIL] (Q.INST [`qs`|->`h::t`] 
-        (RW [AND_IMP_INTRO] (SPEC_ALL SUBSET_seq_addresses_LEMMA))))
-    \\ FULL_SIMP_TAC bool_ss [LENGTH]
-    \\ FULL_SIMP_TAC bool_ss [LENGTH,seq_addresses_def],
-    `seq_addresses x (h'::t) SUBSET seq_addresses (z+4w) zs` by ALL_TAC << [
-      `seq_addresses x (h'::t) SUBSET z INSERT seq_addresses (z+4w) zs` by METIS_TAC [seq_addresses_def]
-      \\ Cases_on `z IN seq_addresses x (h'::t)`
-      \\ IMP_RES_TAC IN_seq_addresses_LEMMA THEN1 `F` by METIS_TAC [] << [
-        `z - 4w IN seq_addresses z (h::zs)` by METIS_TAC [SUBSET_DEF]   
-        \\ IMP_RES_TAC SUBSET_seq_addresses_LEMMA2,
-        FULL_SIMP_TAC bool_ss [SUBSET_DEF,IN_INSERT] \\ METIS_TAC []], 
-      `LENGTH zs < 2 ** 30` by (FULL_SIMP_TAC bool_ss [LENGTH] \\ DECIDE_TAC)
-      \\ Q.PAT_ASSUM `seq_addresses x (h'::t) SUBSET seq_addresses z (h::zs)` (fn th => ALL_TAC)
-      \\ Q.PAT_ASSUM `!z.b` IMP_RES_TAC \\ FULL_SIMP_TAC bool_ss [NOT_CONS_NIL]
-      \\ Q.EXISTS_TAC `h::ys` \\ Q.EXISTS_TAC `ts` \\ Q.EXISTS_TAC `xs`
-      \\ REWRITE_TAC [APPEND,wLENGTH_def,LENGTH,ADD1,GSYM word_add_n2w]
-      \\ ASM_REWRITE_TAC [WORD_MULT_CLAUSES]
-      \\ ONCE_REWRITE_TAC [WORD_ADD_COMM]
-      \\ ASM_REWRITE_TAC [GSYM wLENGTH_def]
-      \\ REWRITE_TAC [WORD_SUB_PLUS,WORD_SUB_ADD]]]);
-
-val WR_skip = prove(
-  ``!xs y ys. LENGTH xs < 2**30 ==> 
-              (WR (4w:word32 * wLENGTH xs) y (xs ++ ys) = xs ++ WR (0w:word32) y ys)``,
-  Induct \\ REWRITE_TAC [wLENGTH_def,LENGTH,APPEND,WORD_MULT_CLAUSES]  
-  \\ REPEAT STRIP_TAC \\ `LENGTH xs < 2 ** 30` by DECIDE_TAC
-  \\ Q.PAT_ASSUM `!x.b` IMP_RES_TAC
-  \\ Q.PAT_ASSUM `!x.b` (fn th => REWRITE_TAC [GSYM th])
-  \\ REWRITE_TAC [WR_def,word_mul_n2w,wLENGTH_def]
-  \\ `4 * SUC (LENGTH xs) < 2 ** 32 /\ 4 * LENGTH xs < 2 ** 32` by 
-    (ASM_REWRITE_TAC [EVAL ``2**32``,GSYM (EVAL ``4 * 2**30``),LT_MULT_LCANCEL,EVAL ``0<4``])
-  \\ FULL_SIMP_TAC (std_ss++SIZES_ss) [w2n_n2w,LESS_MOD] 
-  \\ REWRITE_TAC [MATCH_MP (RW1 [MULT_COMM] MULT_DIV) (DECIDE ``0 < 4``)]
-  \\ REWRITE_TAC [REPLACE_def]);
-
-val RD_skip = prove(
-  ``!xs y ys. LENGTH xs < 2**30 ==> 
-              (RD (4w:word32 * wLENGTH xs) (xs ++ ys) = RD (0w:word32) ys)``,
-  Induct \\ REWRITE_TAC [wLENGTH_def,LENGTH,APPEND,WORD_MULT_CLAUSES]  
-  \\ REPEAT STRIP_TAC \\ `LENGTH xs < 2 ** 30` by DECIDE_TAC
-  \\ Q.PAT_ASSUM `!x.b` IMP_RES_TAC
-  \\ Q.PAT_ASSUM `!x.b` (fn th => REWRITE_TAC [GSYM th])
-  \\ REWRITE_TAC [RD_def,word_mul_n2w,wLENGTH_def]
-  \\ `4 * SUC (LENGTH xs) < 2 ** 32 /\ 4 * LENGTH xs < 2 ** 32` by 
-    (ASM_REWRITE_TAC [EVAL ``2**32``,GSYM (EVAL ``4 * 2**30``),LT_MULT_LCANCEL,EVAL ``0<4``])
-  \\ FULL_SIMP_TAC (std_ss++SIZES_ss) [w2n_n2w,LESS_MOD] 
-  \\ REWRITE_TAC [MATCH_MP (RW1 [MULT_COMM] MULT_DIV) (DECIDE ``0 < 4``)]
-  \\ REWRITE_TAC [EL,TL]);
-
-val seq_APPEND = prove(
-  ``!xs ys a. seq a (xs ++ ys) = seq a xs * seq (a + 4w * wLENGTH xs) ys``,
-  Induct 
-  \\ ASM_REWRITE_TAC [APPEND,seq_def,emp_STAR,wLENGTH_def,LENGTH,WORD_ADD_0,WORD_MULT_CLAUSES]
-  \\ SIMP_TAC bool_ss [ADD1,AC WORD_ADD_ASSOC WORD_ADD_COMM,GSYM word_add_n2w,
-      WORD_MULT_CLAUSES,STAR_ASSOC]);
-
-val IMP_seq_LESS_LEMMA = prove(
-  ``!n xs. ~(LENGTH xs <= n) ==> ?zs y ys. (xs = zs ++ y::ys) /\ (LENGTH zs = n)``,
-  Induct \\ Cases \\ REWRITE_TAC [LENGTH,LESS_EQ_REFL] \\ REPEAT STRIP_TAC
-  THEN1 (Q.EXISTS_TAC `[]` \\ REWRITE_TAC [CONS_11,LENGTH,APPEND] \\ METIS_TAC [])
-  THEN1 `F` by DECIDE_TAC
-  \\ FULL_SIMP_TAC bool_ss [ADD1,LE_ADD_RCANCEL]
-  \\ Q.PAT_ASSUM `!x.b` IMP_RES_TAC \\ ASM_REWRITE_TAC []
-  \\ Q.EXISTS_TAC `h::zs` \\ Q.EXISTS_TAC `y` \\ Q.EXISTS_TAC `ys`
-  \\ ASM_REWRITE_TAC [APPEND,ADD1,LENGTH]);
-
-val IMP_seq_LESS = prove(
-  ``(LENGTH xs <= 2**30 ==> ARM_PROG (P * seq x xs) code C Q Z) ==>
-    ARM_PROG (P * seq x xs) code C Q Z``,
-  REPEAT STRIP_TAC \\ Cases_on `LENGTH xs <= 2**30` THEN1 METIS_TAC []
-  \\ IMP_RES_TAC IMP_seq_LESS_LEMMA
-  \\ ASM_REWRITE_TAC [seq_APPEND,wLENGTH_def,word_mul_n2w]
-  \\ ONCE_REWRITE_TAC [GSYM n2w_mod]
-  \\ FULL_SIMP_TAC (std_ss++SIZES_ss) [WORD_ADD_0]
-  \\ Cases_on `zs` THEN1 (FULL_SIMP_TAC bool_ss [LENGTH] \\ `F` by DECIDE_TAC)   
-  \\ REWRITE_TAC [seq_def,STAR_ASSOC]
-  \\ MOVE_STAR_TAC `p*m1*q1*m2*q2` `m1*m2*(q1*q2*p)`
-  \\ REWRITE_TAC [ARM_PROG_M_11]);
-
-val WR_RD = prove(
-  ``!x zs. WR x (RD x zs) zs = zs``,
-  REWRITE_TAC [WR_def,RD_def] \\ Cases_word \\ ASM_SIMP_TAC bool_ss [w2n_n2w,LESS_MOD]
-  \\ POP_ASSUM (fn th => ALL_TAC) \\ Q.SPEC_TAC (`n DIV 4`,`n`) \\ Induct
-  \\ Cases \\ ASM_REWRITE_TAC [REPLACE_def,EL,HD,TL]);
-
-val list_WR_SNOC = prove(
-  ``!x q qs xs. list_WR x (SNOC q qs) xs = list_WR x qs (WR (x + 4w * wLENGTH qs) q xs)``,
-  Induct_on `qs`
-  THEN1 REWRITE_TAC [SNOC_APPEND,wLENGTH_def,LENGTH,APPEND,WORD_ADD_0,list_WR_def,WORD_MULT_CLAUSES]
-  \\ ASM_REWRITE_TAC [SNOC,list_WR_def,wLENGTH_def,ADD1,LENGTH,
-       WORD_MULT_CLAUSES,GSYM word_add_n2w,WORD_ADD_ASSOC]);
-
-val ARM_PROG_INTRO_SEQ_LIST_WR_LEMMA = prove(
-  ``!qs xs ys zs. 
-      (LENGTH ys = LENGTH qs) /\ LENGTH (xs ++ ys ++ zs) <= 2**30 ==>
-      (list_WR (4w:word32 * wLENGTH xs) qs (xs ++ ys ++ zs) = xs ++ qs ++ zs)``,
-  Induct_on `LENGTH qs` \\ REPEAT STRIP_TAC THEN1  
-   (Cases_on `qs` \\ Cases_on `ys` \\ FULL_SIMP_TAC bool_ss [LENGTH,list_WR_def]
-    \\ METIS_TAC [DECIDE ``~(SUC n = 0)``])
-  \\ `(qs = []) \/ ?q qs'. qs = SNOC q qs'` by METIS_TAC [SNOC_CASES] 
-  \\ FULL_SIMP_TAC bool_ss [LENGTH,DECIDE ``~(SUC n = 0)``]
-  \\ `(ys = []) \/ ?y ys'. ys = SNOC y ys'` by METIS_TAC [SNOC_CASES] 
-  \\ FULL_SIMP_TAC bool_ss [LENGTH,DECIDE ``~(SUC n = 0)``,LENGTH_SNOC]
-  \\ REWRITE_TAC [list_WR_SNOC]
-  \\ REWRITE_TAC [SNOC_APPEND,GSYM WORD_LEFT_ADD_DISTRIB,wLENGTH_def,word_add_n2w]
-  \\ `LENGTH qs' = LENGTH ys'` by FULL_SIMP_TAC bool_ss [ADD1,EQ_ADD_RCANCEL]
-  \\ ASM_REWRITE_TAC []
-  \\ REWRITE_TAC [GSYM LENGTH_APPEND,APPEND_ASSOC]
-  \\ FULL_SIMP_TAC bool_ss [LENGTH_APPEND,LENGTH_SNOC]
-  \\ `xs ++ ys' ++ [y] ++ zs = (xs ++ ys') ++ (y::zs)` by REWRITE_TAC [GSYM APPEND_ASSOC,APPEND]
-  \\ ASM_REWRITE_TAC [GSYM LENGTH_APPEND,GSYM wLENGTH_def]
-  \\ `LENGTH (xs ++ ys') < 2**30` by (FULL_SIMP_TAC bool_ss [LENGTH_APPEND] \\ DECIDE_TAC)
-  \\ IMP_RES_TAC WR_skip
-  \\ ASM_REWRITE_TAC []
-  \\ ASM_REWRITE_TAC [WR_def,EVAL ``w2n (0w:word32) DIV 4``,REPLACE_def]
-  \\ REWRITE_TAC [GSYM APPEND_ASSOC,APPEND]
-  \\ REWRITE_TAC [APPEND_ASSOC,APPEND]
-  \\ Q.PAT_ASSUM `!qs''. (v = LENGTH qs'') ==> c` 
-      (MATCH_MP_TAC o RW [AND_IMP_INTRO] o DISCH ``v = LENGTH (ys':'a list)`` o SPEC_ALL o UNDISCH o Q.SPEC `ys'`)  
-  \\ FULL_SIMP_TAC bool_ss [ADD1,EQ_ADD_RCANCEL,LENGTH] \\ DECIDE_TAC);  
- 
-val ARM_PROG_INTRO_SEQ_LIST_RD_LEMMA = prove(
-  ``!qs:'r list xs:'q list ys zs. 
-      (LENGTH ys = LENGTH qs) /\ LENGTH (xs ++ ys ++ zs) <= 2**30 ==>
-      (list_RD (4w:word32 * wLENGTH xs) qs (xs ++ ys ++ zs) = ys)``,
-  Induct
-  THEN1 (STRIP_TAC \\ Cases \\ REWRITE_TAC [LENGTH,list_RD_def,DECIDE ``~(SUC n = 0)``])
-  \\ REPEAT STRIP_TAC
-  \\ Cases_on `ys` \\ FULL_SIMP_TAC bool_ss [LENGTH,DECIDE ``~(0 = SUC n)``]
-  \\ FULL_SIMP_TAC bool_ss [LENGTH_APPEND,LENGTH]
-  \\ `LENGTH xs < 2**30` by DECIDE_TAC
-  \\ ASM_SIMP_TAC bool_ss [list_RD_def,RD_skip,GSYM APPEND_ASSOC]
-  \\ REWRITE_TAC [RD_def,REPLACE_def,EVAL ``w2n (0w:word32) DIV 4``,EL,HD,APPEND,CONS_11] 
-  \\ `4w * wLENGTH xs + 4w = 4w * wLENGTH (xs ++ [h':'q]) : word32` by 
-    (REWRITE_TAC [wLENGTH_def,LENGTH_APPEND,LENGTH,GSYM word_add_n2w,ADD1]
-     \\ REWRITE_TAC [WORD_LEFT_ADD_DISTRIB] \\ REWRITE_TAC [WORD_MULT_CLAUSES,WORD_ADD_0])
-  \\ `xs ++ h'::(t ++ zs) = (xs ++ [h']) ++ t ++ zs` by REWRITE_TAC [APPEND,GSYM APPEND_ASSOC]
-  \\ ASM_REWRITE_TAC []
-  \\ Q.PAT_ASSUM `!xs. b` MATCH_MP_TAC  
-  \\ FULL_SIMP_TAC bool_ss [ADD1,LENGTH_APPEND,LENGTH,EQ_ADD_RCANCEL] \\ DECIDE_TAC);
-
-val seq_EQ_ms = prove(
-  ``!xs x. seq x xs = ms (addr30 x) xs``,
-  Induct \\ ASM_REWRITE_TAC [seq_def,ms_def] \\ STRIP_TAC \\ Cases_word
-  \\ REWRITE_TAC [addr30_n2w,word_add_n2w,
-   (RW1 [ADD_COMM] o RW [MULT_CLAUSES] o Q.SPEC `1` o MATCH_MP ADD_DIV_ADD_DIV o DECIDE) ``0 < 4``]);
-
-val IN_seq_addresses_SEP_CONTAINS = prove(
-  ``!zs z x. x IN ms_address_set z (LENGTH zs) ==> 
-             ?y. SEP_CONTAINS (byte x y) (ms z zs)``,
-  Induct \\ REWRITE_TAC [ms_address_set_def,NOT_IN_EMPTY,IN_INSERT,LENGTH]
-  \\ REPEAT STRIP_TAC \\ ASM_REWRITE_TAC [] 
-  \\ REWRITE_TAC [ms_def,M_def,SEP_CONTAINS_def]
-  THEN1 (MOVE_STAR_TAC `a1*a2*a3*a4*m` `a4*(a1*a2*a3*m)` \\ METIS_TAC [])
-  THEN1 (MOVE_STAR_TAC `a1*a2*a3*a4*m` `a3*(a1*a2*a4*m)` \\ METIS_TAC [])
-  THEN1 (MOVE_STAR_TAC `a1*a2*a3*a4*m` `a2*(a1*a3*a4*m)` \\ METIS_TAC [])
-  THEN1 (MOVE_STAR_TAC `a1*a2*a3*a4*m` `a1*(a2*a3*a4*m)` \\ METIS_TAC [])
-  \\ Q.PAT_ASSUM `!x.b` IMP_RES_TAC
-  \\ Q.EXISTS_TAC `y` \\ FULL_SIMP_TAC bool_ss [SEP_CONTAINS_def]
-  \\ MOVE_STAR_TAC `a1*a2*a3*a4*(b*m)` `b*(a1*a2*a3*a4*m)` \\ METIS_TAC []);
-      
-val SEQ_IMP_LENGTH_LESS = prove(
-  ``(LENGTH zs < 2**30 ==> ARM_PROG (P * seq z zs) [code] {} Q {}) ==>
-    (ARM_PROG (P * seq z zs) [code] {} Q {})``,
-  Cases_on `LENGTH zs < 2 ** 30` \\ ASM_REWRITE_TAC []
-  \\ REWRITE_TAC [GSYM ((RW [EVAL ``SUC 0 <= 2**30``,LENGTH] o Q.SPECL [`P`,`[c]`]) ARM_PROG_INTRO1)]
-  \\ REWRITE_TAC [ms_def,emp_STAR,seq_EQ_ms,M_def] \\ REPEAT STRIP_TAC
-  \\ FULL_SIMP_TAC bool_ss [DECIDE ``~(n < m) = m <= n:num``]       
-  \\ IMP_RES_TAC FORALL_IN_ms_address_set
-  \\ Q.PAT_ASSUM `!x.b` (ASSUME_TAC o Q.SPECL [`addr30 z`,`addr32 p + 3w`])
-  \\ IMP_RES_TAC IN_seq_addresses_SEP_CONTAINS
-  \\ FULL_SIMP_TAC bool_ss [SEP_CONTAINS_def]
-  \\ MOVE_STAR_TAC `p*(b*f)*(b1*b2*b3*b4)*t` `b*b1*(p*b2*b3*b4*t*f)`
-  \\ REWRITE_TAC [RW [SEP_DISJ_CLAUSES] (Q.SPECL[`P`,`SEP_F`] ARM_RUN_byte_11)]
-  \\ REWRITE_TAC [ARM_RUN_def,RUN_FALSE_PRE]);
-
-val seq_addresses_SUBSET_IMP = prove(
-  ``seq_addresses x qs SUBSET seq_addresses z zs /\ LENGTH (zs:word32 list) < 2**30 ==>
-    LENGTH (qs:'a list) < 2**30``,
-  REWRITE_TAC [SUBSET_DEF] \\ REPEAT STRIP_TAC
-  \\ `~(z - 4w IN seq_addresses z zs)` by METIS_TAC [LENGTH_LESS_EQ_NOT_IN_seq_addresses]  
-  \\ CCONTR_TAC  \\ `z - 4w IN seq_addresses x qs` by ALL_TAC
-  THENL [ALL_TAC,METIS_TAC []] \\ FULL_SIMP_TAC bool_ss [DECIDE ``~(n<m)=m<=n:num``]
-  \\ REWRITE_TAC [IN_seq_addresses2]    
-  \\ Cases_on `qs` \\ FULL_SIMP_TAC bool_ss [LENGTH,EVAL ``2**30 <= 0``] 
-  \\ `x IN seq_addresses z zs` by METIS_TAC [IN_INSERT,seq_addresses_def]
-  \\ `?k. (x = z + n2w (4 * k)) /\ k < LENGTH zs` by METIS_TAC [IN_seq_addresses2]
-  \\ ASM_REWRITE_TAC [] \\ ASM_REWRITE_TAC [WORD_EQ_SUB_RADD]
-  \\ Q.EXISTS_TAC `2**30 - (k + 1)` \\ STRIP_TAC THENL [ALL_TAC,DECIDE_TAC]
-  \\ `!x y q. z + x + y + q = z + y + (x + q)` by SIMP_TAC bool_ss [AC WORD_ADD_ASSOC WORD_ADD_COMM]
-  \\ ONCE_ASM_REWRITE_TAC []
-  \\ REWRITE_TAC [RW [WORD_ADD_0] (Q.SPECL [`k`,`0w`] WORD_EQ_ADD_LCANCEL),GSYM WORD_ADD_ASSOC]
-  \\ REWRITE_TAC [word_add_n2w]    
-  \\ Q.PAT_ASSUM `!x y.b` (fn th => ALL_TAC)
-  \\ REWRITE_TAC [DECIDE ``4*k + 4 = 4 * (k + 1)``]  
-  \\ REWRITE_TAC [GSYM LEFT_ADD_DISTRIB]
-  \\ `k + 1 <= 2**30` by DECIDE_TAC
-  \\ ASM_SIMP_TAC bool_ss [SUB_ADD,n2w_11] \\ EVAL_TAC);
-
-val ARM_PROG_INTRO_SEQ_LIST_WR = prove(
-  ``(!ys. (LENGTH ys = LENGTH qs) ==> 
-          ARM_PROG2 c (P * ms (addr30 x) ys) [code] (Q * ms (addr30 x) qs) {}) ==>
-    ARM_PROG2 c (P * seq z zs * cond (seq_addresses x qs SUBSET seq_addresses z zs)) [code]  
-                (Q * seq z (list_WR (x-z) qs zs)) {}``,
-  REWRITE_TAC [ARM_PROG_MOVE_COND,ARM_PROG2_def] 
-  \\ ONCE_REWRITE_TAC [CONJ_COMM] \\ REPEAT STRIP_TAC THEN1 METIS_TAC []
-  \\ MATCH_MP_TAC SEQ_IMP_LENGTH_LESS \\ STRIP_TAC
-  \\ IMP_RES_TAC seq_addresses_SUBSET_IMP
-  \\ IMP_RES_TAC SUBSET_seq_addresses \\ ASM_REWRITE_TAC []
-  THEN1 (FULL_SIMP_TAC bool_ss [list_WR_def,LENGTH,LENGTH_NIL,ms_def,emp_STAR]     
-         \\ METIS_TAC [ARM_PROG_FRAME,setSTAR_CLAUSES])
-  \\ IMP_RES_TAC LESS_IMP_LESS_OR_EQ    
-  \\ `LENGTH (ys ++ ts ++ xs) <= 2**30 /\ (LENGTH ts = LENGTH qs)` by METIS_TAC []
-  \\ IMP_RES_TAC ARM_PROG_INTRO_SEQ_LIST_WR_LEMMA
-  \\ Q.PAT_ASSUM `4w * wLENGTH ys = x - z` (ASSUME_TAC o GSYM) 
-  \\ ASM_REWRITE_TAC []
-  \\ REWRITE_TAC [seq_APPEND]
-  \\ ONCE_REWRITE_TAC [WORD_ADD_COMM]
-  \\ Q.PAT_ASSUM `x - z = 4w * wLENGTH ys` (fn th => REWRITE_TAC [GSYM th])
-  \\ SIMP_TAC bool_ss [WORD_SUB_ADD,wLENGTH_def,LENGTH_APPEND]
-  \\ Q.PAT_ASSUM `LENGTH ts = LENGTH qs` (fn th => REWRITE_TAC [th])
-  \\ MOVE_STAR_TAC `p*(z*x*w)` `p*x*(z*w)`
-  \\ REWRITE_TAC [seq_EQ_ms]  
-  \\ METIS_TAC [ARM_PROG_FRAME,setSTAR_CLAUSES]);
-
-val ARM_PROG_INTRO_SEQ_LIST_RD = prove(
-  ``(!ys. (LENGTH ys = LENGTH (qs:'q list)) ==> 
-          (ARM_PROG2:^(ty_antiq ARM_PROG2_type)) c (P * ms (addr30 x) ys) [code] (Q ys * ms (addr30 x) ys) {}) ==>
-    (ARM_PROG2:^(ty_antiq ARM_PROG2_type)) c (P * seq z zs * cond (seq_addresses x qs SUBSET seq_addresses z zs)) [code]  
-                (Q (list_RD (x-z) qs zs) * seq z zs) {}``,
-  REWRITE_TAC [ARM_PROG_MOVE_COND,ARM_PROG2_def] 
-  \\ ONCE_REWRITE_TAC [CONJ_COMM] \\ REPEAT STRIP_TAC 
-  THEN1 (POP_ASSUM (ASSUME_TAC o Q.SPEC `MAP (\x.0w) (qs:'q list)`)
-         \\ FULL_SIMP_TAC bool_ss [LENGTH_MAP])
-  \\ MATCH_MP_TAC SEQ_IMP_LENGTH_LESS \\ STRIP_TAC
-  \\ IMP_RES_TAC seq_addresses_SUBSET_IMP
-  \\ IMP_RES_TAC SUBSET_seq_addresses \\ ASM_REWRITE_TAC []
-  THEN1 (FULL_SIMP_TAC bool_ss [list_RD_def,LENGTH,LENGTH_NIL,ms_def,emp_STAR]     
-         \\ METIS_TAC [ARM_PROG_FRAME,setSTAR_CLAUSES])
-  \\ IMP_RES_TAC LESS_IMP_LESS_OR_EQ    
-  \\ `LENGTH (ys ++ ts ++ xs) <= 2**30 /\ (LENGTH ts = LENGTH qs)` by METIS_TAC []
-  \\ IMP_RES_TAC ARM_PROG_INTRO_SEQ_LIST_RD_LEMMA  \\ Q.PAT_ASSUM `4w * wLENGTH ys = x - z` (ASSUME_TAC o GSYM) 
-  \\ ASM_REWRITE_TAC []
-  \\ REWRITE_TAC [seq_APPEND]
-  \\ ONCE_REWRITE_TAC [WORD_ADD_COMM]
-  \\ Q.PAT_ASSUM `x - z = 4w * wLENGTH ys` (fn th => REWRITE_TAC [GSYM th])
-  \\ SIMP_TAC bool_ss [WORD_SUB_ADD,wLENGTH_def,LENGTH_APPEND]
-  \\ Q.PAT_ASSUM `LENGTH ts = LENGTH qs` (fn th => REWRITE_TAC [th])
-  \\ MOVE_STAR_TAC `p*(z*x*w)` `p*x*(z*w)`
-  \\ REWRITE_TAC [seq_EQ_ms]  
-  \\ METIS_TAC [ARM_PROG_FRAME,setSTAR_CLAUSES]);
-
-val ARM_PROG_INTRO_SEQ_RD = prove(
-  ``(!y. ARM_PROG2 c (P * M (addr30 x) y) code (Q y * M (addr30 x) y) {}) ==>
-    ARM_PROG2 c (P * seq z zs * cond (x IN seq_addresses z zs)) code  
-                (Q (RD (x-z) zs) * seq z zs) {}``,
-  REWRITE_TAC [ARM_PROG_MOVE_COND,ARM_PROG2_def] 
-  \\ ONCE_REWRITE_TAC [CONJ_COMM] \\ REPEAT STRIP_TAC THEN1 METIS_TAC []
-  \\ IMP_RES_TAC IN_seq_addresses \\ ASM_REWRITE_TAC []
-  \\ ONCE_REWRITE_TAC [GSYM (REWRITE_CONV [APPEND] ``[x] ++ xs``)]  
-  \\ MATCH_MP_TAC IMP_seq_LESS 
-  \\ REWRITE_TAC [LENGTH_APPEND,LENGTH,ADD1,ADD] \\ STRIP_TAC  
-  \\ `LENGTH ys < 2**30` by DECIDE_TAC \\ IMP_RES_TAC RD_skip \\ IMP_RES_TAC WR_skip
-  \\ Q.PAT_ASSUM `4w * wLENGTH ys = rrr` 
-       (fn th => ASM_REWRITE_TAC [GSYM th] THEN ASSUME_TAC th)
-  \\ REWRITE_TAC [WR_def,RD_def,EVAL ``w2n (0w:word32)``,EVAL ``0 DIV 4``,APPEND,EL,HD,REPLACE_def]  
-  \\ ASM_REWRITE_TAC [seq_APPEND,seq_def]
-  \\ ONCE_REWRITE_TAC [WORD_ADD_COMM] \\ REWRITE_TAC [WORD_SUB_ADD]
-  \\ MOVE_STAR_TAC `p*(s*(m*q))` `p*m*(s*q)`
-  \\ METIS_TAC [ARM_PROG_FRAME,setSTAR_CLAUSES]);
-
-val ARM_PROG_INTRO_SEQ_RD_WR = prove(
-  ``(!y. ARM_PROG2 c (P * M (addr30 x) y) code (Q y * M (addr30 x) q) {}) ==>
-    ARM_PROG2 c (P * seq z zs * cond (x IN seq_addresses z zs)) code  
-                (Q (RD (x-z) zs) * seq z (WR (x-z) q zs)) {}``,
-  REWRITE_TAC [ARM_PROG_MOVE_COND,ARM_PROG2_def] 
-  \\ ONCE_REWRITE_TAC [CONJ_COMM] \\ REPEAT STRIP_TAC THEN1 METIS_TAC []
-  \\ IMP_RES_TAC IN_seq_addresses \\ ASM_REWRITE_TAC []
-  \\ ONCE_REWRITE_TAC [GSYM (REWRITE_CONV [APPEND] ``[x] ++ xs``)]  
-  \\ MATCH_MP_TAC IMP_seq_LESS 
-  \\ REWRITE_TAC [LENGTH_APPEND,LENGTH,ADD1,ADD] \\ STRIP_TAC  
-  \\ `LENGTH ys < 2**30` by DECIDE_TAC \\ IMP_RES_TAC RD_skip \\ IMP_RES_TAC WR_skip
-  \\ Q.PAT_ASSUM `4w * wLENGTH ys = rrr` 
-       (fn th => ASM_REWRITE_TAC [GSYM th] THEN ASSUME_TAC th)
-  \\ REWRITE_TAC [WR_def,RD_def,EVAL ``w2n (0w:word32)``,EVAL ``0 DIV 4``,APPEND,EL,HD,REPLACE_def]  
-  \\ ASM_REWRITE_TAC [seq_APPEND,seq_def]
-  \\ ONCE_REWRITE_TAC [WORD_ADD_COMM] \\ REWRITE_TAC [WORD_SUB_ADD]
-  \\ MOVE_STAR_TAC `p*(s*(m*q))` `p*m*(s*q)`
-  \\ METIS_TAC [ARM_PROG_FRAME,setSTAR_CLAUSES]);
-
-val ARM_PROG_INTRO_SEQ_WR = 
-  SIMP_RULE std_ss [] (Q.INST [`Q`|->`\x. Q`] ARM_PROG_INTRO_SEQ_RD_WR);
-*)
 
 
 (* ----------------------------------------------------------------------------- *)
@@ -907,8 +421,13 @@ val REG_WRITE_READ = prove(
 (* address mode 1 *)
 
 val _ = Hol_datatype `
-  abbrev_addr1 = OneReg | Imm of word8 | 
-                 RegLSR of word5 | RegLSL of word5 | RegASR of word5 | RegROR of word5`;
+  abbrev_addr1 = OneReg | 
+                 Imm of word8 | 
+                 DpImm of word4 # word8 |
+                 RegLSR of word5 | 
+                 RegLSL of word5 | 
+                 RegASR of word5 | 
+                 RegROR of word5`;
 
 val ADDR_MODE1_CMD_def = Define `
   (ADDR_MODE1_CMD OneReg Rd = Dp_shift_immediate (LSL Rd) 0w) /\
@@ -916,11 +435,15 @@ val ADDR_MODE1_CMD_def = Define `
   (ADDR_MODE1_CMD (RegLSL w) Rd = Dp_shift_immediate (LSL Rd) w) /\
   (ADDR_MODE1_CMD (RegASR w) Rd = Dp_shift_immediate (ASR Rd) w) /\
   (ADDR_MODE1_CMD (RegROR w) Rd = Dp_shift_immediate (ROR Rd) w) /\
-  (ADDR_MODE1_CMD (Imm k) Rd = Dp_immediate 0w k)`;
+  (ADDR_MODE1_CMD (Imm k) Rd = Dp_immediate 0w k) /\
+  (ADDR_MODE1_CMD (DpImm (q,r)) Rd = Dp_immediate q r)`;
 
 val ADDR_MODE1_VAL_def = Define `
   (ADDR_MODE1_VAL OneReg  x c = (c,x)) /\
   (ADDR_MODE1_VAL (Imm k) x c = (c,w2w k)) /\
+  (ADDR_MODE1_VAL (DpImm (i,k)) x c = 
+    (FST (IMMEDIATE c ((11 >< 0) (33554432w:word32 !! w2w i << 8 !! w2w k))), 
+     SND (IMMEDIATE c ((11 >< 0) (33554432w:word32 !! w2w i << 8 !! w2w k))))) /\
   (ADDR_MODE1_VAL (RegLSL w) x c = (if w = 0w then c else x %% (32 - w2n w),x << w2n w)) /\
   (ADDR_MODE1_VAL (RegASR w) x c = 
      ((if w = 0w then x %% 31 else x %% (w2n w - 1)),
@@ -938,14 +461,17 @@ val ADDR_MODE1_VAL_THM = prove(
          (IS_DP_IMMEDIATE (ADDR_MODE1_CMD c Rd))
          ((11 >< 0) (addr_mode1_encode (ADDR_MODE1_CMD c Rd))) =
         ADDR_MODE1_VAL c (REG_READ state.registers mode Rd) z``,
-  Cases_on `c`
+  Cases
   \\ REWRITE_TAC [ADDR_MODE1_CMD_def,ADDR_MODE1_VAL_def]
   \\ REWRITE_TAC [IS_DP_IMMEDIATE_def,shift_immediate_shift_register,ADDR_MODE1_def]
   \\ REWRITE_TAC [immediate_enc,shift_immediate_enc]
   THEN1 SRW_TAC [] [ROR_def,w2w_def,LSL_def,LSR_def,word_mul_n2w]
   THEN1 SRW_TAC [] [ROR_def,w2w_def,LSL_def,LSR_def,word_mul_n2w]
-  \\ Q.SPEC_TAC (`c'`,`c`) \\ Cases_word
+  \\ Q.SPEC_TAC (`c'`,`c`)
+  THENL [ALL_TAC,Cases_word,Cases_word,Cases_word,Cases_word]
   \\ ASM_SIMP_TAC bool_ss [n2w_11,LESS_MOD,ZERO_LT_dimword,w2w_def,w2n_n2w] << [
+    Cases_on `p` \\ SIMP_TAC (srw_ss()) [ADDR_MODE1_CMD_def,IS_DP_IMMEDIATE_def,
+      addr_mode1_encode_def,PAIR,ADDR_MODE1_VAL_def],
     Cases_on `n = 0` 
     \\ ASM_REWRITE_TAC [LSR_def,EVAL ``32w:word8 = 0w``,EVAL ``w2n (32w:word8) - 1``] 
     \\ REWRITE_TAC [WORD_LS,LESS_EQ_REFL,EVAL ``w2n (32w:word8)``]
@@ -1389,7 +915,6 @@ val xM_list_thm = prove(
       DISJOINT x y /\ x UNION y SUBSET z = y SUBSET z DIFF x /\ x SUBSET z` by
         (SRW_TAC [] [SUBSET_DEF,DISJOINT_DEF,EXTENSION] \\ METIS_TAC [])
   \\ REPEAT STRIP_TAC \\ Cases_on `h` \\ Cases_on `p` \\ Cases_on `r`
-
   \\ SIMP_TAC bool_ss [MAP,ALL_DISJOINT_def,pairTheory.FST,xM_list_sem_def,xM_list_def,
                        xM_list_addresses_def,xM_list_address_set_def,FOLDR]
   \\ FULL_SIMP_TAC bool_ss [GSYM xM_list_address_set_def]
@@ -2604,7 +2129,7 @@ val arm_LDM = store_thm("arm_LDM",
       xR_list (MAP (\x.(FST x,NONE)) xs) * 
       ms (ADDR_MODE4_ADDR a_mode x xs) (reg_values xs) * S (sN,sZ,sC,sV) * 
       PASS c_flag (sN,sZ,sC,sV)) 
-     [enc (LDM c_flag F (ADDR_MODE4_CMD a_mode) a (reg_bitmap (MAP FST xs)))]
+     [enc (LDM c_flag F (ADDR_MODE4_CMD a_mode) a (reg_bitmap (MAP FST xs)))] {}
      (R30 a (ADDR_MODE4_WB a_mode x xs) *
       xR_list (MAP (\x.(FST x,SOME (SND x))) xs) *
       ms (ADDR_MODE4_ADDR a_mode x xs) (reg_values xs) * S (sN,sZ,sC,sV)
@@ -2638,7 +2163,7 @@ val arm_LDM_SEQ_THM = prove(
     (ARM_PROG2:^(ty_antiq ARM_PROG2_type)) c_flag
      (R a x * xR_list (MAP (\x.(x,NONE)) xs) * S (sN,sZ,sC,sV) * cond (x && 3w = 0w) *
       PASS c_flag (sN,sZ,sC,sV) * ms (addr30 (ADDR_MODE4_ADDR32 a_mode x xs)) ys) 
-     [enc (LDM c_flag F (ADDR_MODE4_CMD a_mode) a (reg_bitmap xs))]
+     [enc (LDM c_flag F (ADDR_MODE4_CMD a_mode) a (reg_bitmap xs))] {}
      ((\ys. R a (ADDR_MODE4_WB32 a_mode x xs) *
       xR_list (MAP (\x.(FST x,SOME (SND x))) (ZIP (QSORT $<=+ xs,ys))) *
       S (sN,sZ,sC,sV)) ys * ms (addr30 (ADDR_MODE4_ADDR32 a_mode x xs)) ys
@@ -2693,7 +2218,7 @@ val arm_LDM_ADDR = store_thm("arm_LDM_ADDR",
      (R30 a x * xR_list (MAP (\x.(FST x,NONE)) xs) * 
       ms (ADDR_MODE4_ADDR a_mode x ((a,y)::xs)) (reg_values ((a,y)::xs)) * S (sN,sZ,sC,sV) * 
       PASS c_flag (sN,sZ,sC,sV)) 
-     [enc (LDM c_flag F (ADDR_MODE4_CMD a_mode) a (reg_bitmap (a::MAP FST xs)))]
+     [enc (LDM c_flag F (ADDR_MODE4_CMD a_mode) a (reg_bitmap (a::MAP FST xs)))] {}
      (xR_list (MAP (\x.(FST x,SOME (SND x))) ((a,y)::xs)) *
       ms (ADDR_MODE4_ADDR a_mode x ((a,y)::xs)) (reg_values ((a,y)::xs)) * S (sN,sZ,sC,sV)
        :^(ty_antiq ARMel_type) set -> bool) {}``,
@@ -2732,7 +2257,7 @@ val arm_LDM_PC = store_thm("arm_LDM_PC",
       xR_list (MAP (\x.(FST x,NONE)) xs) * 
       ms (ADDR_MODE4_ADDR a_mode x ((15w,addr32 p)::xs)) 
          (reg_values ((15w,addr32 p)::xs)) * S (sN,sZ,sC,sV) * PASS c_flag (sN,sZ,sC,sV)) 
-     [enc (LDM c_flag F (ADDR_MODE4_CMD a_mode) a (reg_bitmap (15w :: MAP FST xs)))] SEP_F
+     [enc (LDM c_flag F (ADDR_MODE4_CMD a_mode) a (reg_bitmap (15w :: MAP FST xs)))] {} SEP_F
      {(R30 a (ADDR_MODE4_WB a_mode x ((15w,addr32 p)::xs)) *
        xR_list (MAP (\x.(FST x,SOME (SND x))) xs) *
        ms (ADDR_MODE4_ADDR a_mode x ((15w,addr32 p)::xs)) (reg_values ((15w,addr32 p)::xs)) * 
@@ -2772,7 +2297,7 @@ val arm_LDM_PC_ADDR = store_thm("arm_LDM_PC_ADDR",
       xR_list (MAP (\x.(FST x,NONE)) xs) * 
       ms (ADDR_MODE4_ADDR a_mode x ((15w,addr32 p)::(a,y)::xs)) 
          (reg_values ((15w,addr32 p)::(a,y)::xs)) * S (sN,sZ,sC,sV) * PASS c_flag (sN,sZ,sC,sV)) 
-     [enc (LDM c_flag F (ADDR_MODE4_CMD a_mode) a (reg_bitmap (15w :: a :: MAP FST xs)))] SEP_F
+     [enc (LDM c_flag F (ADDR_MODE4_CMD a_mode) a (reg_bitmap (15w :: a :: MAP FST xs)))] {} SEP_F
      {(xR_list (MAP (\x.(FST x,SOME (SND x))) ((a,y)::xs)) *
        ms (ADDR_MODE4_ADDR a_mode x ((15w,addr32 p)::(a,y)::xs)) (reg_values ((15w,addr32 p)::(a,y)::xs)) * 
        S (sN,sZ,sC,sV),pcSET p)}``,
@@ -3196,7 +2721,7 @@ val arm_STM = store_thm("arm_STM",
       xR_list (MAP (\x.(FST x,SOME (SND x))) xs) * 
       blank_ms (ADDR_MODE4_ADDR a_mode x xs) (LENGTH xs) * 
       S (sN,sZ,sC,sV) * PASS c_flag (sN,sZ,sC,sV)) 
-     [enc (STM c_flag F (ADDR_MODE4_CMD a_mode) a (reg_bitmap (MAP FST xs)))]
+     [enc (STM c_flag F (ADDR_MODE4_CMD a_mode) a (reg_bitmap (MAP FST xs)))] {}
      (R30 a (ADDR_MODE4_WB a_mode x xs) *
       xR_list (MAP (\x.(FST x,SOME (SND x))) xs) *
       ms (ADDR_MODE4_ADDR a_mode x xs) (reg_values xs) * S (sN,sZ,sC,sV)) {}``,
@@ -3229,7 +2754,7 @@ val arm_STM_SEQ_THM = prove(
      (R a x * xR_list (MAP (\x.(FST x,SOME (SND x))) xs) * 
       S (sN,sZ,sC,sV) * PASS c_flag (sN,sZ,sC,sV) * cond (x && 3w = 0w) *
       ms (addr30 (ADDR_MODE4_ADDR32 a_mode x xs)) ys) 
-     [enc (STM c_flag F (ADDR_MODE4_CMD a_mode) a (reg_bitmap (MAP FST xs)))]
+     [enc (STM c_flag F (ADDR_MODE4_CMD a_mode) a (reg_bitmap (MAP FST xs)))] {}
      (R a (ADDR_MODE4_WB32 a_mode x xs) *
       xR_list (MAP (\x.(FST x,SOME (SND x))) xs) * S (sN,sZ,sC,sV) * 
       ms (addr30 (ADDR_MODE4_ADDR32 a_mode x xs)) (reg_values xs)) {}``,
@@ -3634,7 +3159,7 @@ val arm_LDRB = store_thm("arm_LDRB",
   ``(ARM_PROG2:^(ty_antiq ARM_PROG2_type)) c_flag 
      (R a x * R b y * byte (ADDR_MODE2_ADDR' opt imm y) z * S (sN,sZ,sC,sV) *
       PASS c_flag (sN,sZ,sC,sV))
-     [enc (LDR c_flag T opt a b (Dt_immediate imm))]
+     [enc (LDR c_flag T opt a b (Dt_immediate imm))] {}
      (R a (w2w z) * R b (ADDR_MODE2_WB' opt imm y) * byte (ADDR_MODE2_ADDR' opt imm y) z *
       S (sN,sZ,sC,sV)) {}``,
   ARM_PROG2_INIT_TAC ARM_LDR_NOP
@@ -3650,7 +3175,7 @@ val arm_LDRB1 = store_thm("arm_LDRB1",
   ``(ARM_PROG2:^(ty_antiq ARM_PROG2_type)) c_flag 
      (R b x * byte (ADDR_MODE2_ADDR' opt imm x) z * cond ~opt.Wb * S (sN,sZ,sC,sV) *
       PASS c_flag (sN,sZ,sC,sV))
-     [enc (LDR c_flag T opt b b (Dt_immediate imm))]
+     [enc (LDR c_flag T opt b b (Dt_immediate imm))] {}
      (R b (w2w z) * byte (ADDR_MODE2_ADDR' opt imm x) z * S (sN,sZ,sC,sV)) {}``,
   ARM_PROG2_INIT_TAC ARM_LDR_NOP
       `a*m*cd'*st*cd*cmd*pc*ud` `a*pc*cmd*m*st*ud*cd'*cd`
@@ -3659,6 +3184,138 @@ val arm_LDRB1 = store_thm("arm_LDRB1",
   \\ ASSUME_TAC (UNDISCH_ALL (simple_clean ldrb1 []))
   \\ ARM_PROG2_HAMMER_TAC);
 
+val ldr_pc = FIX_ADDR_MODE2 `F` ARM_LDR_PC
+val ldr_pc = (UNDISCH_ALL o Q.INST [`Rd`|->`a`,`c`|->`c_flag`] o DISCH_ALL) ldr_pc
+
+val w2w_and_3 = prove(
+   ``!i. ((i:word12) && 3w = 0w) ==> ((w2w i) && 3w:word32 = 0w)``,
+   Cases_word
+   \\ `n MOD 4 < 4` by METIS_TAC [DIVISION,DECIDE ``0<4``]
+   \\ `n MOD 4 < 4096` by DECIDE_TAC
+   \\ `n MOD 4 < 4294967296` by DECIDE_TAC
+   \\ ASM_SIMP_TAC (std_ss++SIZES_ss) [n2w_and_3,w2w_def,w2n_n2w,n2w_11,LESS_MOD]); 
+
+val arm_LDR_PC_ADDRESS = prove(
+  ``addr30 (if opt.Up then addr32 p + 8w + w2w imm else addr32 p + 8w - w2w imm) =
+    pcADD (addr30 (if opt.Up then 8w + w2w imm else 8w - w2w imm)) p``,
+  Cases_on `opt.Up` 
+  \\ ASM_SIMP_TAC std_ss [addr30_addr32_ADD,GSYM WORD_ADD_ASSOC,word_sub_def,pcADD_def,
+       AC WORD_ADD_COMM WORD_ADD_ASSOC]);
+
+val arm_LDR_PC_LEMMA1 = prove(
+  ``ARM_RUN (M (I p) (enc (LDR c_flag F opt a 15w (Dt_immediate imm))) *
+             M (pcADD(addr30 (if opt.Up then 8w + w2w imm else 8w - w2w imm)) p) y *
+             R a x * R 15w (addr32 p) * 
+             S (sN,sZ,sC,sV) * one (Undef F) * cond (opt.Pre /\ ~opt.Wb /\ (imm && 3w = 0w)) * 
+             cond (CONDITION_PASSED2 (sN,sZ,sC,sV) c_flag))
+            (M (I p) (enc (LDR c_flag F opt a 15w (Dt_immediate imm))) *
+             M (pcADD(addr30 (if opt.Up then 8w + w2w imm else 8w - w2w imm)) p) y *
+             R a y * R 15w (addr32 (pcADD 1w p)) * 
+             S (sN,sZ,sC,sV) * one (Undef F))``,
+  SIMP_TAC (std_ss++sep2_ss) [ARM_RUN_SEMANTICS,GSYM arm_LDR_PC_ADDRESS] 
+  \\ SIMP_TAC std_ss [RW1 [WORD_ADD_COMM] pcADD_def]
+  \\ REPEAT STRIP_TAC
+  \\ Q.EXISTS_TAC `1` \\ SIMP_TAC std_ss [STATE_ARM_MEM_1,LET_DEF]
+  \\ ASM_MOVE_STAR_TAC `m1*m2*ra*pc*ss*oo*c` `ra*pc*m1*m2*ss*oo*c`
+  \\ MOVE_STAR_TAC `m1*m2*ra*pc*ss*oo` `ra*pc*m1*m2*ss*oo`
+  \\ ARM_PROG2_EXPAND_TAC xR2 xMmm
+  \\ ASSUME_TAC (UNDISCH_ALL (simple_clean ldr_pc []))
+  \\ `(status (NEXT_ARM_MEM s) = status s) /\ ~(NEXT_ARM_MEM s).undefined` by 
+    ASM_SIMP_TAC (srw_ss()) [status_def,statusN_def,statusZ_def,statusC_def,statusV_def]
+  \\ `!x. mem x (NEXT_ARM_MEM s) = mem x s` by ASM_SIMP_TAC (srw_ss()) [mem_def]
+  \\ `owrt_visible (NEXT_ARM_MEM s) = owrt_visible s` by 
+    ASM_SIMP_TAC (srw_ss()) [owrt_visible_def,set_status_def,
+                             owrt_visible_regs_def,REG_OWRT_ALL,state_mode_def]
+ \\ `!b. reg b (NEXT_ARM_MEM s) = if b = 15w then addr32 (p+1w) else if b = a then y else reg b s` by 
+   (ASM_SIMP_TAC (srw_ss()) [reg_def,state_mode_def] \\ STRIP_TAC
+    \\ Cases_on `b = 15w` \\ ASM_SIMP_TAC bool_ss [] << [      
+      REWRITE_TAC [REG_READ6_def,FETCH_PC_def,GSYM INC_PC]
+      \\ ASM_SIMP_TAC bool_ss [REG_WRITE_INC_PC,INC_PC_r15,REG_WRITE_r15]
+      \\ FULL_SIMP_TAC std_ss [reg_def,addr32_ADD,addr32_n2w],
+      Cases_on `b = a` \\ ASM_SIMP_TAC bool_ss [REG_READ_WRITE_NEQ]
+      \\ FULL_SIMP_TAC bool_ss [REG_READ_WRITE,GSYM state_mode_def,reg_def]
+      \\ FULL_SIMP_TAC bool_ss [REG_READ_def]
+      \\ Q.PAT_ASSUM `NEXT_ARM_MEM s = dgd` (fn th => ALL_TAC)     
+      \\ `(1 >< 0) (ADDR_MODE2_ADDR' opt imm (addr32 p + 8w)) = 0w:word2` by 
+       (Cases_on `opt.Up` \\ ASM_SIMP_TAC bool_ss [ADDR_MODE2_ADDR'_def]
+        \\ REWRITE_TAC [GSYM (SIMP_CONV std_ss [addr32_n2w] ``addr32 2w``)]
+        \\ IMP_RES_TAC w2w_and_3
+        \\ IMP_RES_TAC EXISTS_addr30
+        \\ ASM_SIMP_TAC std_ss [GSYM addr32_ADD,GSYM addr32_SUB,addr32_eq_0])
+      \\ ASM_SIMP_TAC std_ss [EVAL ``w2n (0w:word2)``,SHIFT_ZERO,ADDR_MODE2_ADDR'_def]])    
+  \\ Q.PAT_ASSUM `NEXT_ARM_MEM s = dgd` (fn th => ALL_TAC)     
+  \\ ASM_SIMP_TAC bool_ss []
+  \\ Q.ABBREV_TAC `nnn = addr30 (if opt.Up then addr32 p + 8w + w2w imm else addr32 p + 8w - w2w imm)`
+  \\ ASM_SIMP_TAC std_ss [arm2set''_EQ,IN_INSERT,NOT_IN_EMPTY,mem_byte_def]);
+
+val arm_LDR_PC_LEMMA2 = prove(
+  ``(I p = pcADD (addr30 (if opt.Up then 8w + w2w imm else 8w - w2w imm)) p) /\
+    (enc (LDR c_flag F opt a 15w (Dt_immediate imm)) = y) ==>
+    ARM_RUN (M (I p) (enc (LDR c_flag F opt a 15w (Dt_immediate imm))) *
+             R a x * R 15w (addr32 p) * 
+             S (sN,sZ,sC,sV) * one (Undef F) * cond (opt.Pre /\ ~opt.Wb /\ (imm && 3w = 0w)) * 
+             cond (CONDITION_PASSED2 (sN,sZ,sC,sV) c_flag))
+            (M (I p) (enc (LDR c_flag F opt a 15w (Dt_immediate imm))) *
+             R a y * R 15w (addr32 (pcADD 1w p)) * 
+             S (sN,sZ,sC,sV) * one (Undef F))``,
+  SIMP_TAC (std_ss++sep2_ss) [ARM_RUN_SEMANTICS,GSYM arm_LDR_PC_ADDRESS] 
+  \\ SIMP_TAC std_ss [RW1 [WORD_ADD_COMM] pcADD_def]
+  \\ CONV_TAC ((RATOR_CONV o RAND_CONV o RATOR_CONV) (ONCE_REWRITE_CONV [EQ_SYM_EQ]))
+  \\ SIMP_TAC (std_ss++sep2_ss) [ARM_RUN_SEMANTICS,GSYM arm_LDR_PC_ADDRESS] 
+  \\ REPEAT STRIP_TAC
+  \\ Q.EXISTS_TAC `1` \\ SIMP_TAC std_ss [STATE_ARM_MEM_1,LET_DEF]
+  \\ ASM_MOVE_STAR_TAC `m1*ra*pc*ss*oo*c` `ra*pc*m1*ss*oo*c`
+  \\ MOVE_STAR_TAC `m1*ra*pc*ss*oo` `ra*pc*m1*ss*oo`
+  \\ ARM_PROG2_EXPAND_TAC xR2 xMm
+  \\ `mem (addr30 (reg 15w s)) s = enc (LDR c_flag F opt a 15w (Dt_immediate imm))` by METIS_TAC []
+  \\ ASSUME_TAC (UNDISCH_ALL (simple_clean ldr_pc []))
+  \\ `(status (NEXT_ARM_MEM s) = status s) /\ ~(NEXT_ARM_MEM s).undefined` by 
+    ASM_SIMP_TAC (srw_ss()) [status_def,statusN_def,statusZ_def,statusC_def,statusV_def]
+  \\ `!x. mem x (NEXT_ARM_MEM s) = mem x s` by ASM_SIMP_TAC (srw_ss()) [mem_def]
+  \\ `owrt_visible (NEXT_ARM_MEM s) = owrt_visible s` by 
+    ASM_SIMP_TAC (srw_ss()) [owrt_visible_def,set_status_def,
+                             owrt_visible_regs_def,REG_OWRT_ALL,state_mode_def]
+  \\ `!b. reg b (NEXT_ARM_MEM s) = if b = 15w then addr32 (p+1w) else if b = a then y else reg b s` by 
+   (ASM_SIMP_TAC (srw_ss()) [reg_def,state_mode_def] \\ STRIP_TAC
+    \\ Cases_on `b = 15w` \\ ASM_SIMP_TAC bool_ss [] << [      
+      REWRITE_TAC [REG_READ6_def,FETCH_PC_def,GSYM INC_PC]
+      \\ ASM_SIMP_TAC bool_ss [REG_WRITE_INC_PC,INC_PC_r15,REG_WRITE_r15]
+      \\ FULL_SIMP_TAC std_ss [reg_def,addr32_ADD,addr32_n2w],
+      Cases_on `b = a` \\ ASM_SIMP_TAC bool_ss [REG_READ_WRITE_NEQ]
+      \\ FULL_SIMP_TAC bool_ss [REG_READ_WRITE,GSYM state_mode_def,reg_def]
+      \\ FULL_SIMP_TAC bool_ss [REG_READ_def]
+      \\ Q.PAT_ASSUM `NEXT_ARM_MEM s = dgd` (fn th => ALL_TAC)     
+      \\ `(1 >< 0) (ADDR_MODE2_ADDR' opt imm (addr32 p + 8w)) = 0w:word2` by 
+       (Cases_on `opt.Up` \\ ASM_SIMP_TAC bool_ss [ADDR_MODE2_ADDR'_def]
+        \\ REWRITE_TAC [GSYM (SIMP_CONV std_ss [addr32_n2w] ``addr32 2w``)]
+        \\ IMP_RES_TAC w2w_and_3
+        \\ IMP_RES_TAC EXISTS_addr30
+        \\ ASM_SIMP_TAC std_ss [GSYM addr32_ADD,GSYM addr32_SUB,addr32_eq_0])
+      \\ ASM_SIMP_TAC std_ss [EVAL ``w2n (0w:word2)``,SHIFT_ZERO,ADDR_MODE2_ADDR'_def]])    
+  \\ Q.PAT_ASSUM `NEXT_ARM_MEM s = dgd` (fn th => ALL_TAC)     
+  \\ ASM_SIMP_TAC bool_ss []
+  \\ Q.ABBREV_TAC `nnn = addr30 (if opt.Up then addr32 p + 8w + w2w imm else addr32 p + 8w - w2w imm)`
+  \\ ASM_SIMP_TAC std_ss [arm2set''_EQ,IN_INSERT,NOT_IN_EMPTY,mem_byte_def]);
+
+val lemma = MATCH_MP (RW [GSYM STAR_ASSOC] IMP_ARM_RUN_mpool) (RW [GSYM STAR_ASSOC] arm_LDR_PC_LEMMA1)
+val lemma = MATCH_MP lemma (RW [GSYM STAR_ASSOC] arm_LDR_PC_LEMMA2)
+val lemma = RW [STAR_ASSOC] lemma
+    
+val arm_LDR_PC_NONALIGNED = store_thm("arm_LDR_PC_NONALIGNED",
+  ``(ARM_PROG2:^(ty_antiq ARM_PROG2_type)) c_flag
+     (R a x * S (sN,sZ,sC,sV) * PASS c_flag (sN,sZ,sC,sV) * 
+      cond (opt.Pre /\ ~opt.Wb /\ (imm && 3w = 0w)))
+     [enc (LDR c_flag F opt a 15w (Dt_immediate imm))]
+     {([y],pcADD (addr30 (if opt.Up then 8w + w2w imm else 8w - w2w imm)))}
+     (R a y * S (sN,sZ,sC,sV)) {}``,
+  REWRITE_TAC [ARM_PROG2_def] \\ REPEAT STRIP_TAC
+  THENL [ALL_TAC,METIS_TAC [MAKE_ARM_NOP ARM_LDR_NOP,UNION_EMPTY,ARM_PROG_ADD_CODE]]
+  \\ SIMP_TAC std_ss [ARM_PROG_THM,ARM_GPROG_THM,GPROG_DISJ_CLAUSES,PASS_def,R30_def,
+                      pcINC_def,wLENGTH_def,LENGTH,ARMpc_def,STAR_ASSOC]
+  \\ STRIP_TAC \\ ASSUME_TAC lemma
+  \\ FULL_SIMP_TAC (std_ss) [AC WORD_ADD_ASSOC WORD_ADD_COMM,
+       AC CONJ_COMM CONJ_ASSOC, AC STAR_ASSOC STAR_COMM]);
+
 val ldr = FIX_ADDR_MODE2 `F` ARM_LDR
 val ldr = (UNDISCH_ALL o Q.INST [`Rd`|->`a`,`Rn`|->`b`,`c`|->`c_flag`] o DISCH_ALL) ldr
 
@@ -3666,7 +3323,7 @@ val arm_LDR_NONALIGNED = store_thm("arm_LDR_NONALIGNED",
   ``(ARM_PROG2:^(ty_antiq ARM_PROG2_type)) c_flag
      (R a x * R b y * M (addr30 (ADDR_MODE2_ADDR' opt imm y)) z *
       S (sN,sZ,sC,sV) * PASS c_flag (sN,sZ,sC,sV))
-     [enc (LDR c_flag F opt a b (Dt_immediate imm))]
+     [enc (LDR c_flag F opt a b (Dt_immediate imm))] {}
      (R a (z #>> (8 * w2n (((1 >< 0) ((ADDR_MODE2_ADDR' opt imm y))):word2))) *
       R b (ADDR_MODE2_WB' opt imm y) *
       M (addr30 (ADDR_MODE2_ADDR' opt imm y)) z * S (sN,sZ,sC,sV)) {}``,
@@ -3682,7 +3339,7 @@ val arm_LDR_SEQ_LEMMA = prove(
      (R a x * R b y * S (sN,sZ,sC,sV) * PASS c_flag (sN,sZ,sC,sV) * 
       cond (ADDR_MODE2_ADDR' opt imm y && 3w = 0w) * 
       M (addr30 (ADDR_MODE2_ADDR' opt imm y)) z)
-     [enc (LDR c_flag F opt a b (Dt_immediate imm))]
+     [enc (LDR c_flag F opt a b (Dt_immediate imm))] {}
      ((\z. R a z * R b (ADDR_MODE2_WB' opt imm y) * S (sN,sZ,sC,sV)) z *
       M (addr30 (ADDR_MODE2_ADDR' opt imm y)) z) {}``,
   SIMP_TAC std_ss []
@@ -3705,7 +3362,7 @@ val arm_LDR1_NONALIGNED = store_thm("arm_LDR1_NONALIGNED",
   ``(ARM_PROG2:^(ty_antiq ARM_PROG2_type)) c_flag
      (R b y * M (addr30 (ADDR_MODE2_ADDR' opt imm y)) z * cond ~opt.Wb * S (sN,sZ,sC,sV) *
       PASS c_flag (sN,sZ,sC,sV))
-     [enc (LDR c_flag F opt b b (Dt_immediate imm))]
+     [enc (LDR c_flag F opt b b (Dt_immediate imm))] {}
      (R b (z #>> (8 * w2n (((1 >< 0) (ADDR_MODE2_ADDR' opt imm y)):word2))) *
       M (addr30 (ADDR_MODE2_ADDR' opt imm y)) z * S (sN,sZ,sC,sV)) {}``,
   ARM_PROG2_INIT_TAC ARM_LDR_NOP
@@ -3720,7 +3377,7 @@ val arm_LDR1_SEQ_LEMMA = prove(
      (R b y * S (sN,sZ,sC,sV) * PASS c_flag (sN,sZ,sC,sV) * cond ~opt.Wb *
       cond (ADDR_MODE2_ADDR' opt imm y && 3w = 0w) * 
       M (addr30 (ADDR_MODE2_ADDR' opt imm y)) z)
-     [enc (LDR c_flag F opt b b (Dt_immediate imm))]
+     [enc (LDR c_flag F opt b b (Dt_immediate imm))] {}
      ((\z. R b z * S (sN,sZ,sC,sV)) z *
       M (addr30 (ADDR_MODE2_ADDR' opt imm y)) z) {}``,
   SIMP_TAC std_ss []
@@ -3747,7 +3404,7 @@ val arm_LDR_PC = store_thm("arm_LDR_PC",
   ``(ARM_PROG2:^(ty_antiq ARM_PROG2_type)) c_flag
      (R30 a x * M (ADDR_MODE2_ADDR opt imm x) (addr32 y) * S (sN,sZ,sC,sV) *
       PASS c_flag (sN,sZ,sC,sV))
-     [enc (LDR c_flag F opt 15w a (Dt_immediate ((w2w (imm:word8)) << 2)))]
+     [enc (LDR c_flag F opt 15w a (Dt_immediate ((w2w (imm:word8)) << 2)))] {}
      SEP_F
      {(R30 a (ADDR_MODE2_WB opt imm x) * 
        M (ADDR_MODE2_ADDR opt imm x) (addr32 y) * S (sN,sZ,sC,sV),pcSET y)}``,
@@ -3808,7 +3465,7 @@ val arm_STRB = store_thm("arm_STRB",
   ``(ARM_PROG2:^(ty_antiq ARM_PROG2_type)) c_flag 
      (R a x * R b y * byte (ADDR_MODE2_ADDR' opt imm y) z * S (sN,sZ,sC,sV) *
       PASS c_flag (sN,sZ,sC,sV))
-     [enc (STR c_flag T opt a b (Dt_immediate imm))]
+     [enc (STR c_flag T opt a b (Dt_immediate imm))] {}
      (R a x * R b (ADDR_MODE2_WB' opt imm y) * byte (ADDR_MODE2_ADDR' opt imm y) ((7 >< 0) x) *
       S (sN,sZ,sC,sV)) {}``,
   ARM_PROG2_INIT_TAC ARM_STR_NOP
@@ -3859,7 +3516,7 @@ val arm_STR_NONALIGNED = store_thm("arm_STR_NONALIGNED",
   ``(ARM_PROG2:^(ty_antiq ARM_PROG2_type)) c_flag
      (R a x * R b y * M (addr30 (ADDR_MODE2_ADDR' opt imm y)) z *
       S (sN,sZ,sC,sV) * PASS c_flag (sN,sZ,sC,sV))
-     [enc (STR c_flag F opt a b (Dt_immediate imm))]
+     [enc (STR c_flag F opt a b (Dt_immediate imm))] {}
      (R a x * R b (ADDR_MODE2_WB' opt imm y) *
       M (addr30 (ADDR_MODE2_ADDR' opt imm y)) x * S (sN,sZ,sC,sV)) {}``,
   ARM_PROG2_INIT_TAC ARM_STR_NOP
@@ -3892,7 +3549,7 @@ val swpb = (Q.INST [`Rm`|->`a`,`Rd`|->`b`,`Rn`|->`c`,`c`|->`c_flag`] o DISCH_ALL
 val arm_SWPB3 = store_thm("arm_SWPB3",
   ``(ARM_PROG2:^(ty_antiq ARM_PROG2_type)) c_flag
      (R a x * R b y * R c z * byte z q * S (sN,sZ,sC,sV) *
-      PASS c_flag (sN,sZ,sC,sV)) [enc (SWP c_flag T b a c)]
+      PASS c_flag (sN,sZ,sC,sV)) [enc (SWP c_flag T b a c)] {}
      (R a x * R b (w2w q) * R c z * byte z ((7 >< 0) x) * 
       S (sN,sZ,sC,sV)) {}``,
   ARM_PROG2_INIT_TAC ARM_SWP_NOP
@@ -3913,7 +3570,7 @@ val swpb2 = Q.INST [`b`|->`a`,`c`|->`b`] swpb
 val arm_SWPB2 = store_thm("arm_SWPB2",
   ``(ARM_PROG2:^(ty_antiq ARM_PROG2_type)) c_flag
      (R a x * R b y * byte y q * S (sN,sZ,sC,sV) * PASS c_flag (sN,sZ,sC,sV)) 
-     [enc (SWP c_flag T a a b)]
+     [enc (SWP c_flag T a a b)] {}
      (R a (w2w q) * R b y * byte y ((7 >< 0) x) * S (sN,sZ,sC,sV)) {}``,
   ARM_PROG2_INIT_TAC ARM_SWP_NOP
       `a*b*m*st*cd*cmd*pc*ud` `a*b*pc*cmd*m*st*ud*cd`
@@ -3935,7 +3592,7 @@ val swp = (Q.INST [`Rm`|->`a`,`Rd`|->`b`,`Rn`|->`c`,`c`|->`c_flag`] o DISCH_ALL)
 val arm_SWP3_NONALIGNED = store_thm("arm_SWP3_NONALIGNED",
   ``(ARM_PROG2:^(ty_antiq ARM_PROG2_type)) c_flag
      (R a x * R b y * R c z * M (addr30 z) q * S (sN,sZ,sC,sV) *
-      PASS c_flag (sN,sZ,sC,sV)) [enc (SWP c_flag F b a c)]
+      PASS c_flag (sN,sZ,sC,sV)) [enc (SWP c_flag F b a c)] {}
      (R a x * R b (q #>> (8 * w2n (((1 >< 0) z):word2))) * R c z *
       M (addr30 z) x * S (sN,sZ,sC,sV)) {}``,
   ARM_PROG2_INIT_TAC ARM_SWP_NOP
@@ -3953,7 +3610,7 @@ val arm_SWP3_NONALIGNED = store_thm("arm_SWP3_NONALIGNED",
 val arm_SWP3_SEQ_LEMMA = prove(
   ``!q. (ARM_PROG2:^(ty_antiq ARM_PROG2_type)) c_flag
      (R a x * R b y * R c z * S (sN,sZ,sC,sV) * cond (z && 3w = 0w) *
-      PASS c_flag (sN,sZ,sC,sV) * M (addr30 z) q) [enc (SWP c_flag F b a c)]
+      PASS c_flag (sN,sZ,sC,sV) * M (addr30 z) q) [enc (SWP c_flag F b a c)] {}
      ((\q. R a x * R b q * R c z * S (sN,sZ,sC,sV)) q * 
       M (addr30 z) x) {}``,
   SIMP_TAC std_ss []
@@ -3979,7 +3636,7 @@ val swp2 = Q.INST [`b`|->`a`,`c`|->`b`] swp
 val arm_SWP2_NONALIGNED = store_thm("arm_SWP2_NONALIGNED",
   ``(ARM_PROG2:^(ty_antiq ARM_PROG2_type)) c_flag
      (R a x * R b y * M (addr30 y) q * S (sN,sZ,sC,sV) *
-      PASS c_flag (sN,sZ,sC,sV)) [enc (SWP c_flag F a a b)]
+      PASS c_flag (sN,sZ,sC,sV)) [enc (SWP c_flag F a a b)] {}
      (R a (q #>> (8 * w2n (((1 >< 0) y):word2))) * R b y * M (addr30 y) x *
       S (sN,sZ,sC,sV)) {}``,
   ARM_PROG2_INIT_TAC ARM_SWP_NOP
@@ -3997,7 +3654,7 @@ val arm_SWP2_NONALIGNED = store_thm("arm_SWP2_NONALIGNED",
 val arm_SWP2_SEQ_LEMMA = prove(
   ``!q. (ARM_PROG2:^(ty_antiq ARM_PROG2_type)) c_flag
      (R a x * R b y * S (sN,sZ,sC,sV) * cond (y && 3w = 0w) *
-      PASS c_flag (sN,sZ,sC,sV) * M (addr30 y) q) [enc (SWP c_flag F a a b)]
+      PASS c_flag (sN,sZ,sC,sV) * M (addr30 y) q) [enc (SWP c_flag F a a b)] {}
      ((\q. R a q * R b y * S (sN,sZ,sC,sV)) q * 
       M (addr30 y) x) {}``,
   SIMP_TAC std_ss []
@@ -4029,7 +3686,7 @@ fun simple_clean_AM1 s th =
 val arm_CMN1 = store_thm("arm_CMN1",
   ``(ARM_PROG2:^(ty_antiq ARM_PROG2_type)) c_flag
            (R a x * S (sN,sZ,sC,sV) * PASS c_flag (sN,sZ,sC,sV))
-           [enc (CMN c_flag a (ADDR_MODE1_CMD a_mode a))]
+           [enc (CMN c_flag a (ADDR_MODE1_CMD a_mode a))] {}
            (R a x *
             S
               (word_msb (x + SND (ADDR_MODE1_VAL a_mode x sC)),
@@ -4047,7 +3704,7 @@ val arm_CMN1 = store_thm("arm_CMN1",
 val arm_CMN2 = store_thm("arm_CMN2",
   ``(ARM_PROG2:^(ty_antiq ARM_PROG2_type)) c_flag
            (R a x * R b y * S (sN,sZ,sC,sV) * PASS c_flag (sN,sZ,sC,sV))
-           [enc (CMN c_flag a (ADDR_MODE1_CMD a_mode b))]
+           [enc (CMN c_flag a (ADDR_MODE1_CMD a_mode b))] {}
            (R a x * R b y *
             S
               (word_msb (x + SND (ADDR_MODE1_VAL a_mode y sC)),
@@ -4065,7 +3722,7 @@ val arm_CMN2 = store_thm("arm_CMN2",
 val arm_CMP1 = store_thm("arm_CMP1",
   ``(ARM_PROG2:^(ty_antiq ARM_PROG2_type)) c_flag
            (R a x * S (sN,sZ,sC,sV) * PASS c_flag (sN,sZ,sC,sV))
-           [enc (CMP c_flag a (ADDR_MODE1_CMD a_mode a))]
+           [enc (CMP c_flag a (ADDR_MODE1_CMD a_mode a))] {}
            (R a x *
             S
               (word_msb (x - SND (ADDR_MODE1_VAL a_mode x sC)),
@@ -4083,7 +3740,7 @@ val arm_CMP1 = store_thm("arm_CMP1",
 val arm_CMP2 = store_thm("arm_CMP2",
   ``(ARM_PROG2:^(ty_antiq ARM_PROG2_type)) c_flag
            (R a x * R b y * S (sN,sZ,sC,sV) * PASS c_flag (sN,sZ,sC,sV))
-           [enc (CMP c_flag a (ADDR_MODE1_CMD a_mode b))]
+           [enc (CMP c_flag a (ADDR_MODE1_CMD a_mode b))] {}
            (R a x * R b y *
             S
               (word_msb (x - SND (ADDR_MODE1_VAL a_mode y sC)),
@@ -4101,7 +3758,7 @@ val arm_CMP2 = store_thm("arm_CMP2",
 val arm_TST1 = store_thm("arm_TST1",
   ``(ARM_PROG2:^(ty_antiq ARM_PROG2_type)) c_flag
            (R a x * S (sN,sZ,sC,sV) * PASS c_flag (sN,sZ,sC,sV))
-           [enc (TST c_flag a (ADDR_MODE1_CMD a_mode a))]
+           [enc (TST c_flag a (ADDR_MODE1_CMD a_mode a))] {}
            (R a x *
             S
               (word_msb (x && SND (ADDR_MODE1_VAL a_mode x sC)),
@@ -4117,7 +3774,7 @@ val arm_TST1 = store_thm("arm_TST1",
 val arm_TST2 = store_thm("arm_TST2",
   ``(ARM_PROG2:^(ty_antiq ARM_PROG2_type)) c_flag
            (R a x * R b y * S (sN,sZ,sC,sV) * PASS c_flag (sN,sZ,sC,sV))
-           [enc (TST c_flag a (ADDR_MODE1_CMD a_mode b))]
+           [enc (TST c_flag a (ADDR_MODE1_CMD a_mode b))] {}
            (R a x * R b y *
             S
               (word_msb (x && SND (ADDR_MODE1_VAL a_mode y sC)),
@@ -4133,7 +3790,7 @@ val arm_TST2 = store_thm("arm_TST2",
 val arm_TEQ1 = store_thm("arm_TEQ1",
   ``(ARM_PROG2:^(ty_antiq ARM_PROG2_type)) c_flag
            (R a x * S (sN,sZ,sC,sV) * PASS c_flag (sN,sZ,sC,sV))
-           [enc (TEQ c_flag a (ADDR_MODE1_CMD a_mode a))]
+           [enc (TEQ c_flag a (ADDR_MODE1_CMD a_mode a))] {}
            (R a x *
             S
               (word_msb (x ?? SND (ADDR_MODE1_VAL a_mode x sC)),
@@ -4149,7 +3806,7 @@ val arm_TEQ1 = store_thm("arm_TEQ1",
 val arm_TEQ2 = store_thm("arm_TEQ2",
   ``(ARM_PROG2:^(ty_antiq ARM_PROG2_type)) c_flag
            (R a x * R b y * S (sN,sZ,sC,sV) * PASS c_flag (sN,sZ,sC,sV))
-           [enc (TEQ c_flag a (ADDR_MODE1_CMD a_mode b))]
+           [enc (TEQ c_flag a (ADDR_MODE1_CMD a_mode b))] {}
            (R a x * R b y *
             S
               (word_msb (x ?? SND (ADDR_MODE1_VAL a_mode y sC)),
@@ -4170,7 +3827,7 @@ val arm_TEQ2 = store_thm("arm_TEQ2",
 val arm_MOV1 = store_thm("arm_MOV1",
   ``(ARM_PROG2:^(ty_antiq ARM_PROG2_type)) c_flag
            (R a x * S (sN,sZ,sC,sV) * PASS c_flag (sN,sZ,sC,sV))
-           [enc (MOV c_flag s_flag a (ADDR_MODE1_CMD a_mode a))]
+           [enc (MOV c_flag s_flag a (ADDR_MODE1_CMD a_mode a))] {}
            (R a (SND (ADDR_MODE1_VAL a_mode x sC)) *
             S
               ((if s_flag then word_msb (SND (ADDR_MODE1_VAL a_mode x sC)) else sN),
@@ -4187,7 +3844,7 @@ val arm_MOV1 = store_thm("arm_MOV1",
 val arm_MOV2 = store_thm("arm_MOV2",
   ``(ARM_PROG2:^(ty_antiq ARM_PROG2_type)) c_flag
            (R a x * R b y * S (sN,sZ,sC,sV) * PASS c_flag (sN,sZ,sC,sV))
-           [enc (MOV c_flag s_flag b (ADDR_MODE1_CMD a_mode a))]
+           [enc (MOV c_flag s_flag b (ADDR_MODE1_CMD a_mode a))] {}
            (R a x * R b (SND (ADDR_MODE1_VAL a_mode x sC)) *
             S
               ((if s_flag then word_msb (SND (ADDR_MODE1_VAL a_mode x sC)) else sN),
@@ -4204,7 +3861,7 @@ val arm_MOV2 = store_thm("arm_MOV2",
 val arm_MVN1 = store_thm("arm_MVN1",
   ``(ARM_PROG2:^(ty_antiq ARM_PROG2_type)) c_flag
            (R a x * S (sN,sZ,sC,sV) * PASS c_flag (sN,sZ,sC,sV))
-           [enc (MVN c_flag s_flag a (ADDR_MODE1_CMD a_mode a))]
+           [enc (MVN c_flag s_flag a (ADDR_MODE1_CMD a_mode a))] {}
            (R a ~SND (ADDR_MODE1_VAL a_mode x sC) *
             S
               ((if s_flag then word_msb ~SND (ADDR_MODE1_VAL a_mode x sC) else sN),
@@ -4221,7 +3878,7 @@ val arm_MVN1 = store_thm("arm_MVN1",
 val arm_MVN2 = store_thm("arm_MVN2",
   ``(ARM_PROG2:^(ty_antiq ARM_PROG2_type)) c_flag
            (R a x * R b y * S (sN,sZ,sC,sV) * PASS c_flag (sN,sZ,sC,sV))
-           [enc (MVN c_flag s_flag b (ADDR_MODE1_CMD a_mode a))]
+           [enc (MVN c_flag s_flag b (ADDR_MODE1_CMD a_mode a))] {}
            (R a x * R b ~SND (ADDR_MODE1_VAL a_mode x sC) *
             S
               ((if s_flag then word_msb ~SND (ADDR_MODE1_VAL a_mode x sC) else sN),
@@ -4243,7 +3900,7 @@ val arm_MVN2 = store_thm("arm_MVN2",
 val arm_MUL3 = store_thm("arm_MUL3",
   ``(ARM_PROG2:^(ty_antiq ARM_PROG2_type)) c_flag
            (R a x * R b y * R c z * S (sN,sZ,sC,sV) * PASS c_flag (sN,sZ,sC,sV))
-           [enc (MUL c_flag s_flag c a b)]
+           [enc (MUL c_flag s_flag c a b)] {}
            (R a x * R b y * R c (x * y) *
             S
               ((if s_flag then word_msb (x * y) else sN),
@@ -4260,7 +3917,7 @@ val arm_MUL3 = store_thm("arm_MUL3",
 val arm_MUL2 = store_thm("arm_MUL2",
   ``(ARM_PROG2:^(ty_antiq ARM_PROG2_type)) c_flag
            (R a x * R b y * S (sN,sZ,sC,sV) * PASS c_flag (sN,sZ,sC,sV))
-           [enc (MUL c_flag s_flag b a b)]
+           [enc (MUL c_flag s_flag b a b)] {}
            (R a x * R b (x * y) *
             S
               ((if s_flag then word_msb (x * y) else sN),
@@ -4277,7 +3934,7 @@ val arm_MUL2 = store_thm("arm_MUL2",
 val arm_MUL2'' = store_thm("arm_MUL2''",
   ``(ARM_PROG2:^(ty_antiq ARM_PROG2_type)) c_flag
            (R a x * R b y * S (sN,sZ,sC,sV) * PASS c_flag (sN,sZ,sC,sV))
-           [enc (MUL c_flag s_flag b a a)]
+           [enc (MUL c_flag s_flag b a a)] {}
            (R a x * R b (x * x) *
             S
               ((if s_flag then word_msb (x * x) else sN),
@@ -4294,7 +3951,7 @@ val arm_MUL2'' = store_thm("arm_MUL2''",
 val arm_MLA4 = store_thm("arm_MLA4",
   ``(ARM_PROG2:^(ty_antiq ARM_PROG2_type)) c_flag
            (R a x * R b y * R c k * R d z * S (sN,sZ,sC,sV) *
-            PASS c_flag (sN,sZ,sC,sV)) [enc (MLA c_flag s_flag d a b c)]
+            PASS c_flag (sN,sZ,sC,sV)) [enc (MLA c_flag s_flag d a b c)] {}
            (R a x * R b y * R c k * R d (k + x * y) *
             S
               ((if s_flag then word_msb (k + x * y) else sN),
@@ -4311,7 +3968,7 @@ val arm_MLA4 = store_thm("arm_MLA4",
 val arm_MLA3 = store_thm("arm_MLA3",
   ``(ARM_PROG2:^(ty_antiq ARM_PROG2_type)) c_flag
            (R a x * R b y * R c z * S (sN,sZ,sC,sV) * PASS c_flag (sN,sZ,sC,sV))
-           [enc (MLA c_flag s_flag c a c b)]
+           [enc (MLA c_flag s_flag c a c b)] {}
            (R a x * R b y * R c (y + x * z) *
             S
               ((if s_flag then word_msb (y + x * z) else sN),
@@ -4328,7 +3985,7 @@ val arm_MLA3 = store_thm("arm_MLA3",
 val arm_MLA3' = store_thm("arm_MLA3'",
   ``(ARM_PROG2:^(ty_antiq ARM_PROG2_type)) c_flag
            (R a x * R b y * R c z * S (sN,sZ,sC,sV) * PASS c_flag (sN,sZ,sC,sV))
-           [enc (MLA c_flag s_flag c a b c)]
+           [enc (MLA c_flag s_flag c a b c)] {}
            (R a x * R b y * R c (z + x * y) *
             S
               ((if s_flag then word_msb (z + x * y) else sN),
@@ -4345,7 +4002,7 @@ val arm_MLA3' = store_thm("arm_MLA3'",
 val arm_MLA3'' = store_thm("arm_MLA3''",
   ``(ARM_PROG2:^(ty_antiq ARM_PROG2_type)) c_flag
            (R a x * R b y * R c z * S (sN,sZ,sC,sV) * PASS c_flag (sN,sZ,sC,sV))
-           [enc (MLA c_flag s_flag c a a b)]
+           [enc (MLA c_flag s_flag c a a b)] {}
            (R a x * R b y * R c (y + x * x) *
             S
               ((if s_flag then word_msb (y + x * x) else sN),
@@ -4368,7 +4025,7 @@ val arm_MLA3'' = store_thm("arm_MLA3''",
 val arm_UMULL4 = store_thm("arm_UMULL4",
   ``(ARM_PROG2:^(ty_antiq ARM_PROG2_type)) c_flag
            (R a x * R b y * R c z * R c' z' * S (sN,sZ,sC,sV) *
-            PASS c_flag (sN,sZ,sC,sV)) [enc (UMULL c_flag s_flag c c' a b)]
+            PASS c_flag (sN,sZ,sC,sV)) [enc (UMULL c_flag s_flag c c' a b)] {}
            (R a x * R b y * R c (x * y) * R c' ((63 >< 32) (w2w x * (w2w y):word64)) *
             S
               ((if s_flag then word_msb ((w2w x * w2w y):word64) else sN),
@@ -4386,7 +4043,7 @@ val arm_UMULL4 = store_thm("arm_UMULL4",
 val arm_UMULL3 = store_thm("arm_UMULL3",
   ``(ARM_PROG2:^(ty_antiq ARM_PROG2_type)) c_flag
            (R a x * R c z * R c' z' * S (sN,sZ,sC,sV) * PASS c_flag (sN,sZ,sC,sV))
-           [enc (UMULL c_flag s_flag c c' a c)]
+           [enc (UMULL c_flag s_flag c c' a c)] {}
            (R a x * R c (x * z) * R c' ((63 >< 32) ((w2w x * w2w z):word64)) *
             S
               ((if s_flag then word_msb ((w2w x * w2w z):word64) else sN),
@@ -4404,7 +4061,7 @@ val arm_UMULL3 = store_thm("arm_UMULL3",
 val arm_UMULL3' = store_thm("arm_UMULL3'",
   ``(ARM_PROG2:^(ty_antiq ARM_PROG2_type)) c_flag
            (R a x * R c z * R c' z' * S (sN,sZ,sC,sV) * PASS c_flag (sN,sZ,sC,sV))
-           [enc (UMULL c_flag s_flag c c' a c')]
+           [enc (UMULL c_flag s_flag c c' a c')] {}
            (R a x * R c (x * z') * R c' ((63 >< 32) ((w2w x * w2w z'):word64)) *
             S
               ((if s_flag then word_msb ((w2w x * w2w z'):word64) else sN),
@@ -4422,7 +4079,7 @@ val arm_UMULL3' = store_thm("arm_UMULL3'",
 val arm_UMULL3'' = store_thm("arm_UMULL3''",
   ``(ARM_PROG2:^(ty_antiq ARM_PROG2_type)) c_flag
            (R a x * R c z * R c' z' * S (sN,sZ,sC,sV) * PASS c_flag (sN,sZ,sC,sV))
-           [enc (UMULL c_flag s_flag c c' a a)]
+           [enc (UMULL c_flag s_flag c c' a a)] {}
            (R a x * R c (x * x) * R c' ((63 >< 32) ((w2w x * w2w x):word64)) *
             S
               ((if s_flag then word_msb ((w2w x * w2w x):word64) else sN),
@@ -4440,7 +4097,7 @@ val arm_UMULL3'' = store_thm("arm_UMULL3''",
 val arm_SMULL4 = store_thm("arm_SMULL4",
   ``(ARM_PROG2:^(ty_antiq ARM_PROG2_type)) c_flag
            (R a x * R b y * R c z * R c' z' * S (sN,sZ,sC,sV) *
-            PASS c_flag (sN,sZ,sC,sV)) [enc (SMULL c_flag s_flag c c' a b)]
+            PASS c_flag (sN,sZ,sC,sV)) [enc (SMULL c_flag s_flag c c' a b)] {}
            (R a x * R b y * R c ((31 >< 0) ((sw2sw x * sw2sw y):word64)) *
             R c' ((63 >< 32) ((sw2sw x * sw2sw y):word64)) *
             S
@@ -4459,7 +4116,7 @@ val arm_SMULL4 = store_thm("arm_SMULL4",
 val arm_SMULL3 = store_thm("arm_SMULL3",
   ``(ARM_PROG2:^(ty_antiq ARM_PROG2_type)) c_flag
            (R a x * R c z * R c' z' * S (sN,sZ,sC,sV) * PASS c_flag (sN,sZ,sC,sV))
-           [enc (SMULL c_flag s_flag c c' a c)]
+           [enc (SMULL c_flag s_flag c c' a c)] {}
            (R a x * R c ((31 >< 0) ((sw2sw x * sw2sw z):word64)) *
             R c' ((63 >< 32) ((sw2sw x * sw2sw z):word64)) *
             S
@@ -4478,7 +4135,7 @@ val arm_SMULL3 = store_thm("arm_SMULL3",
 val arm_SMULL3' = store_thm("arm_SMULL3'",
   ``(ARM_PROG2:^(ty_antiq ARM_PROG2_type)) c_flag
            (R a x * R c z * R c' z' * S (sN,sZ,sC,sV) * PASS c_flag (sN,sZ,sC,sV))
-           [enc (SMULL c_flag s_flag c c' a c')]
+           [enc (SMULL c_flag s_flag c c' a c')] {}
            (R a x * R c ((31 >< 0) ((sw2sw x * sw2sw z'):word64)) *
             R c' ((63 >< 32) ((sw2sw x * sw2sw z'):word64)) *
             S
@@ -4497,7 +4154,7 @@ val arm_SMULL3' = store_thm("arm_SMULL3'",
 val arm_SMULL3'' = store_thm("arm_SMULL3''",
   ``(ARM_PROG2:^(ty_antiq ARM_PROG2_type)) c_flag
            (R a x * R c z * R c' z' * S (sN,sZ,sC,sV) * PASS c_flag (sN,sZ,sC,sV))
-           [enc (SMULL c_flag s_flag c c' a a)]
+           [enc (SMULL c_flag s_flag c c' a a)] {}
            (R a x * R c ((31 >< 0) ((sw2sw x * sw2sw x):word64)) *
             R c' ((63 >< 32) ((sw2sw x * sw2sw x):word64)) *
             S
@@ -4516,7 +4173,7 @@ val arm_SMULL3'' = store_thm("arm_SMULL3''",
 val arm_UMLAL4 = store_thm("arm_UMLAL4",
   ``(ARM_PROG2:^(ty_antiq ARM_PROG2_type)) c_flag
            (R a x * R b y * R c z * R c' z' * S (sN,sZ,sC,sV) *
-            PASS c_flag (sN,sZ,sC,sV)) [enc (UMLAL c_flag s_flag c c' a b)]
+            PASS c_flag (sN,sZ,sC,sV)) [enc (UMLAL c_flag s_flag c c' a b)] {}
            (R a x * R b y * R c ((31 >< 0) ((z' @@ z + w2w x * w2w y):word64)) * 
             R c' ((63 >< 32) (z' @@ z + w2w x * (w2w y):word64)) *
             S
@@ -4535,7 +4192,7 @@ val arm_UMLAL4 = store_thm("arm_UMLAL4",
 val arm_UMLAL3'' = store_thm("arm_UMLAL3''",
   ``(ARM_PROG2:^(ty_antiq ARM_PROG2_type)) c_flag
            (R a x * R c z * R c' z' * S (sN,sZ,sC,sV) * PASS c_flag (sN,sZ,sC,sV))
-           [enc (UMLAL c_flag s_flag c c' a a)]
+           [enc (UMLAL c_flag s_flag c c' a a)] {}
            (R a x * R c ((31 >< 0) ((z' @@ z + w2w x * w2w x):word64)) * 
             R c' ((63 >< 32) ((z' @@ z + w2w x * w2w x):word64)) *
             S
@@ -4554,7 +4211,7 @@ val arm_UMLAL3'' = store_thm("arm_UMLAL3''",
 val arm_SMLAL4 = store_thm("arm_SMLAL4",
   ``(ARM_PROG2:^(ty_antiq ARM_PROG2_type)) c_flag
            (R a x * R b y * R c z * R c' z' * S (sN,sZ,sC,sV) *
-            PASS c_flag (sN,sZ,sC,sV)) [enc (SMLAL c_flag s_flag c c' a b)]
+            PASS c_flag (sN,sZ,sC,sV)) [enc (SMLAL c_flag s_flag c c' a b)] {}
            (R a x * R b y * R c ((31 >< 0) (z' @@ z + (sw2sw x * sw2sw y):word64)) *
             R c' ((63 >< 32) (z' @@ z + (sw2sw x * sw2sw y):word64)) *
             S
@@ -4573,7 +4230,7 @@ val arm_SMLAL4 = store_thm("arm_SMLAL4",
 val arm_SMLAL3'' = store_thm("arm_SMLAL3''",
   ``(ARM_PROG2:^(ty_antiq ARM_PROG2_type)) c_flag
            (R a x * R c z * R c' z' * S (sN,sZ,sC,sV) * PASS c_flag (sN,sZ,sC,sV))
-           [enc (SMLAL c_flag s_flag c c' a a)]
+           [enc (SMLAL c_flag s_flag c c' a a)] {}
            (R a x * R c ((31 >< 0) ((z' @@ z + sw2sw x * sw2sw x):word64)) *
             R c' ((63 >< 32) ((z' @@ z + sw2sw x * sw2sw x):word64)) *
             S
@@ -4597,7 +4254,7 @@ val arm_SMLAL3'' = store_thm("arm_SMLAL3''",
 val arm_ADC1 = store_thm("arm_ADC1",
   ``(ARM_PROG2:^(ty_antiq ARM_PROG2_type)) c_flag
            (R a x * S (sN,sZ,sC,sV) * PASS c_flag (sN,sZ,sC,sV))
-           [enc (ADC c_flag s_flag a a (ADDR_MODE1_CMD a_mode a))]
+           [enc (ADC c_flag s_flag a a (ADDR_MODE1_CMD a_mode a))] {}
            (R a (x + SND (ADDR_MODE1_VAL a_mode x sC) + (if sC then 1w else 0w)) *
             S
               (if s_flag then
@@ -4624,7 +4281,7 @@ val arm_ADC1 = store_thm("arm_ADC1",
 val arm_ADD1 = store_thm("arm_ADD1",
   ``(ARM_PROG2:^(ty_antiq ARM_PROG2_type)) c_flag
            (R a x * S (sN,sZ,sC,sV) * PASS c_flag (sN,sZ,sC,sV))
-           [enc (ADD c_flag s_flag a a (ADDR_MODE1_CMD a_mode a))]
+           [enc (ADD c_flag s_flag a a (ADDR_MODE1_CMD a_mode a))] {}
            (R a (x + SND (ADDR_MODE1_VAL a_mode x sC)) *
             S
               (if s_flag then
@@ -4646,7 +4303,7 @@ val arm_ADD1 = store_thm("arm_ADD1",
 val arm_AND1 = store_thm("arm_AND1",
   ``(ARM_PROG2:^(ty_antiq ARM_PROG2_type)) c_flag
            (R a x * S (sN,sZ,sC,sV) * PASS c_flag (sN,sZ,sC,sV))
-           [enc (AND c_flag s_flag a a (ADDR_MODE1_CMD a_mode a))]
+           [enc (AND c_flag s_flag a a (ADDR_MODE1_CMD a_mode a))] {}
            (R a (x && SND (ADDR_MODE1_VAL a_mode x sC)) *
             S
               ((if s_flag then
@@ -4666,7 +4323,7 @@ val arm_AND1 = store_thm("arm_AND1",
 val arm_BIC1 = store_thm("arm_BIC1",
   ``(ARM_PROG2:^(ty_antiq ARM_PROG2_type)) c_flag
            (R a x * S (sN,sZ,sC,sV) * PASS c_flag (sN,sZ,sC,sV))
-           [enc (BIC c_flag s_flag a a (ADDR_MODE1_CMD a_mode a))]
+           [enc (BIC c_flag s_flag a a (ADDR_MODE1_CMD a_mode a))] {}
            (R a (x && ~SND (ADDR_MODE1_VAL a_mode x sC)) *
             S
               ((if s_flag then
@@ -4686,7 +4343,7 @@ val arm_BIC1 = store_thm("arm_BIC1",
 val arm_EOR1 = store_thm("arm_EOR1",
   ``(ARM_PROG2:^(ty_antiq ARM_PROG2_type)) c_flag
            (R a x * S (sN,sZ,sC,sV) * PASS c_flag (sN,sZ,sC,sV))
-           [enc (EOR c_flag s_flag a a (ADDR_MODE1_CMD a_mode a))]
+           [enc (EOR c_flag s_flag a a (ADDR_MODE1_CMD a_mode a))] {}
            (R a (x ?? SND (ADDR_MODE1_VAL a_mode x sC)) *
             S
               ((if s_flag then
@@ -4706,7 +4363,7 @@ val arm_EOR1 = store_thm("arm_EOR1",
 val arm_ORR1 = store_thm("arm_ORR1",
   ``(ARM_PROG2:^(ty_antiq ARM_PROG2_type)) c_flag
            (R a x * S (sN,sZ,sC,sV) * PASS c_flag (sN,sZ,sC,sV))
-           [enc (ORR c_flag s_flag a a (ADDR_MODE1_CMD a_mode a))]
+           [enc (ORR c_flag s_flag a a (ADDR_MODE1_CMD a_mode a))] {}
            (R a (x !! SND (ADDR_MODE1_VAL a_mode x sC)) *
             S
               ((if s_flag then
@@ -4726,7 +4383,7 @@ val arm_ORR1 = store_thm("arm_ORR1",
 val arm_RSB1 = store_thm("arm_RSB1",
   ``(ARM_PROG2:^(ty_antiq ARM_PROG2_type)) c_flag
            (R a x * S (sN,sZ,sC,sV) * PASS c_flag (sN,sZ,sC,sV))
-           [enc (RSB c_flag s_flag a a (ADDR_MODE1_CMD a_mode a))]
+           [enc (RSB c_flag s_flag a a (ADDR_MODE1_CMD a_mode a))] {}
            (R a (SND (ADDR_MODE1_VAL a_mode x sC) - x) *
             S
               (if s_flag then
@@ -4749,7 +4406,7 @@ val arm_RSB1 = store_thm("arm_RSB1",
 val arm_RSC1 = store_thm("arm_RSC1",
   ``(ARM_PROG2:^(ty_antiq ARM_PROG2_type)) c_flag
            (R a x * S (sN,sZ,sC,sV) * PASS c_flag (sN,sZ,sC,sV))
-           [enc (RSC c_flag s_flag a a (ADDR_MODE1_CMD a_mode a))]
+           [enc (RSC c_flag s_flag a a (ADDR_MODE1_CMD a_mode a))] {}
            (R a (SND (ADDR_MODE1_VAL a_mode x sC) - x - (if sC then 0w else 1w)) *
             S
               (if s_flag then
@@ -4773,7 +4430,7 @@ val arm_RSC1 = store_thm("arm_RSC1",
 val arm_SBC1 = store_thm("arm_SBC1",
   ``(ARM_PROG2:^(ty_antiq ARM_PROG2_type)) c_flag
            (R a x * S (sN,sZ,sC,sV) * PASS c_flag (sN,sZ,sC,sV))
-           [enc (SBC c_flag s_flag a a (ADDR_MODE1_CMD a_mode a))]
+           [enc (SBC c_flag s_flag a a (ADDR_MODE1_CMD a_mode a))] {}
            (R a (x - SND (ADDR_MODE1_VAL a_mode x sC) - (if sC then 0w else 1w)) *
             S
               (if s_flag then
@@ -4797,7 +4454,7 @@ val arm_SBC1 = store_thm("arm_SBC1",
 val arm_SUB1 = store_thm("arm_SUB1",
   ``(ARM_PROG2:^(ty_antiq ARM_PROG2_type)) c_flag
            (R a x * S (sN,sZ,sC,sV) * PASS c_flag (sN,sZ,sC,sV))
-           [enc (SUB c_flag s_flag a a (ADDR_MODE1_CMD a_mode a))]
+           [enc (SUB c_flag s_flag a a (ADDR_MODE1_CMD a_mode a))] {}
            (R a (x - SND (ADDR_MODE1_VAL a_mode x sC)) *
             S
               (if s_flag then
@@ -4819,7 +4476,7 @@ val arm_SUB1 = store_thm("arm_SUB1",
 val arm_ADC2 = store_thm("arm_ADC2",
   ``(ARM_PROG2:^(ty_antiq ARM_PROG2_type)) c_flag
            (R a x * R b y * S (sN,sZ,sC,sV) * PASS c_flag (sN,sZ,sC,sV))
-           [enc (ADC c_flag s_flag b a (ADDR_MODE1_CMD a_mode b))]
+           [enc (ADC c_flag s_flag b a (ADDR_MODE1_CMD a_mode b))] {}
            (R a x *
             R b (x + SND (ADDR_MODE1_VAL a_mode y sC) + (if sC then 1w else 0w)) *
             S
@@ -4849,7 +4506,7 @@ val arm_ADC2 = store_thm("arm_ADC2",
 val arm_ADD2 = store_thm("arm_ADD2",
   ``(ARM_PROG2:^(ty_antiq ARM_PROG2_type)) c_flag
            (R a x * R b y * S (sN,sZ,sC,sV) * PASS c_flag (sN,sZ,sC,sV))
-           [enc (ADD c_flag s_flag b a (ADDR_MODE1_CMD a_mode b))]
+           [enc (ADD c_flag s_flag b a (ADDR_MODE1_CMD a_mode b))] {}
            (R a x * R b (x + SND (ADDR_MODE1_VAL a_mode y sC)) *
             S
               (if s_flag then
@@ -4871,7 +4528,7 @@ val arm_ADD2 = store_thm("arm_ADD2",
 val arm_AND2 = store_thm("arm_AND2",
   ``(ARM_PROG2:^(ty_antiq ARM_PROG2_type)) c_flag
            (R a x * R b y * S (sN,sZ,sC,sV) * PASS c_flag (sN,sZ,sC,sV))
-           [enc (AND c_flag s_flag b a (ADDR_MODE1_CMD a_mode b))]
+           [enc (AND c_flag s_flag b a (ADDR_MODE1_CMD a_mode b))] {}
            (R a x * R b (x && SND (ADDR_MODE1_VAL a_mode y sC)) *
             S
               ((if s_flag then
@@ -4891,7 +4548,7 @@ val arm_AND2 = store_thm("arm_AND2",
 val arm_BIC2 = store_thm("arm_BIC2",
   ``(ARM_PROG2:^(ty_antiq ARM_PROG2_type)) c_flag
            (R a x * R b y * S (sN,sZ,sC,sV) * PASS c_flag (sN,sZ,sC,sV))
-           [enc (BIC c_flag s_flag b a (ADDR_MODE1_CMD a_mode b))]
+           [enc (BIC c_flag s_flag b a (ADDR_MODE1_CMD a_mode b))] {}
            (R a x * R b (x && ~SND (ADDR_MODE1_VAL a_mode y sC)) *
             S
               ((if s_flag then
@@ -4911,7 +4568,7 @@ val arm_BIC2 = store_thm("arm_BIC2",
 val arm_EOR2 = store_thm("arm_EOR2",
   ``(ARM_PROG2:^(ty_antiq ARM_PROG2_type)) c_flag
            (R a x * R b y * S (sN,sZ,sC,sV) * PASS c_flag (sN,sZ,sC,sV))
-           [enc (EOR c_flag s_flag b a (ADDR_MODE1_CMD a_mode b))]
+           [enc (EOR c_flag s_flag b a (ADDR_MODE1_CMD a_mode b))] {}
            (R a x * R b (x ?? SND (ADDR_MODE1_VAL a_mode y sC)) *
             S
               ((if s_flag then
@@ -4931,7 +4588,7 @@ val arm_EOR2 = store_thm("arm_EOR2",
 val arm_ORR2 = store_thm("arm_ORR2",
   ``(ARM_PROG2:^(ty_antiq ARM_PROG2_type)) c_flag
            (R a x * R b y * S (sN,sZ,sC,sV) * PASS c_flag (sN,sZ,sC,sV))
-           [enc (ORR c_flag s_flag b a (ADDR_MODE1_CMD a_mode b))]
+           [enc (ORR c_flag s_flag b a (ADDR_MODE1_CMD a_mode b))] {}
            (R a x * R b (x !! SND (ADDR_MODE1_VAL a_mode y sC)) *
             S
               ((if s_flag then
@@ -4951,7 +4608,7 @@ val arm_ORR2 = store_thm("arm_ORR2",
 val arm_RSB2 = store_thm("arm_RSB2",
   ``(ARM_PROG2:^(ty_antiq ARM_PROG2_type)) c_flag
            (R a x * R b y * S (sN,sZ,sC,sV) * PASS c_flag (sN,sZ,sC,sV))
-           [enc (RSB c_flag s_flag b a (ADDR_MODE1_CMD a_mode b))]
+           [enc (RSB c_flag s_flag b a (ADDR_MODE1_CMD a_mode b))] {}
            (R a x * R b (SND (ADDR_MODE1_VAL a_mode y sC) - x) *
             S
               (if s_flag then
@@ -4974,7 +4631,7 @@ val arm_RSB2 = store_thm("arm_RSB2",
 val arm_RSC2 = store_thm("arm_RSC2",
   ``(ARM_PROG2:^(ty_antiq ARM_PROG2_type)) c_flag
            (R a x * R b y * S (sN,sZ,sC,sV) * PASS c_flag (sN,sZ,sC,sV))
-           [enc (RSC c_flag s_flag b a (ADDR_MODE1_CMD a_mode b))]
+           [enc (RSC c_flag s_flag b a (ADDR_MODE1_CMD a_mode b))] {}
            (R a x *
             R b (SND (ADDR_MODE1_VAL a_mode y sC) - x - (if sC then 0w else 1w)) *
             S
@@ -4999,7 +4656,7 @@ val arm_RSC2 = store_thm("arm_RSC2",
 val arm_SBC2 = store_thm("arm_SBC2",
   ``(ARM_PROG2:^(ty_antiq ARM_PROG2_type)) c_flag
            (R a x * R b y * S (sN,sZ,sC,sV) * PASS c_flag (sN,sZ,sC,sV))
-           [enc (SBC c_flag s_flag b a (ADDR_MODE1_CMD a_mode b))]
+           [enc (SBC c_flag s_flag b a (ADDR_MODE1_CMD a_mode b))] {}
            (R a x * R b (x - SND (ADDR_MODE1_VAL a_mode y sC) - (if sC then 0w else 1w)) *
             S
               (if s_flag then
@@ -5023,7 +4680,7 @@ val arm_SBC2 = store_thm("arm_SBC2",
 val arm_SUB2 = store_thm("arm_SUB2",
   ``(ARM_PROG2:^(ty_antiq ARM_PROG2_type)) c_flag
            (R a x * R b y * S (sN,sZ,sC,sV) * PASS c_flag (sN,sZ,sC,sV))
-           [enc (SUB c_flag s_flag b a (ADDR_MODE1_CMD a_mode b))]
+           [enc (SUB c_flag s_flag b a (ADDR_MODE1_CMD a_mode b))] {}
            (R a x * R b (x - SND (ADDR_MODE1_VAL a_mode y sC)) *
             S
               (if s_flag then
@@ -5045,7 +4702,7 @@ val arm_SUB2 = store_thm("arm_SUB2",
 val arm_ADC2' = store_thm("arm_ADC2'",
   ``(ARM_PROG2:^(ty_antiq ARM_PROG2_type)) c_flag
            (R a x * R b y * S (sN,sZ,sC,sV) * PASS c_flag (sN,sZ,sC,sV))
-           [enc (ADC c_flag s_flag a a (ADDR_MODE1_CMD a_mode b))]
+           [enc (ADC c_flag s_flag a a (ADDR_MODE1_CMD a_mode b))] {}
            (R a (x + SND (ADDR_MODE1_VAL a_mode y sC) + (if sC then 1w else 0w)) *
             R b y *
             S
@@ -5075,7 +4732,7 @@ val arm_ADC2' = store_thm("arm_ADC2'",
 val arm_ADD2' = store_thm("arm_ADD2'",
   ``(ARM_PROG2:^(ty_antiq ARM_PROG2_type)) c_flag
            (R a x * R b y * S (sN,sZ,sC,sV) * PASS c_flag (sN,sZ,sC,sV))
-           [enc (ADD c_flag s_flag a a (ADDR_MODE1_CMD a_mode b))]
+           [enc (ADD c_flag s_flag a a (ADDR_MODE1_CMD a_mode b))] {}
            (R a (x + SND (ADDR_MODE1_VAL a_mode y sC)) * R b y *
             S
               (if s_flag then
@@ -5097,7 +4754,7 @@ val arm_ADD2' = store_thm("arm_ADD2'",
 val arm_AND2' = store_thm("arm_AND2'",
   ``(ARM_PROG2:^(ty_antiq ARM_PROG2_type)) c_flag
            (R a x * R b y * S (sN,sZ,sC,sV) * PASS c_flag (sN,sZ,sC,sV))
-           [enc (AND c_flag s_flag a a (ADDR_MODE1_CMD a_mode b))]
+           [enc (AND c_flag s_flag a a (ADDR_MODE1_CMD a_mode b))] {}
            (R a (x && SND (ADDR_MODE1_VAL a_mode y sC)) * R b y *
             S
               ((if s_flag then
@@ -5117,7 +4774,7 @@ val arm_AND2' = store_thm("arm_AND2'",
 val arm_BIC2' = store_thm("arm_BIC2'",
   ``(ARM_PROG2:^(ty_antiq ARM_PROG2_type)) c_flag
            (R a x * R b y * S (sN,sZ,sC,sV) * PASS c_flag (sN,sZ,sC,sV))
-           [enc (BIC c_flag s_flag a a (ADDR_MODE1_CMD a_mode b))]
+           [enc (BIC c_flag s_flag a a (ADDR_MODE1_CMD a_mode b))] {}
            (R a (x && ~SND (ADDR_MODE1_VAL a_mode y sC)) * R b y *
             S
               ((if s_flag then
@@ -5137,7 +4794,7 @@ val arm_BIC2' = store_thm("arm_BIC2'",
 val arm_EOR2' = store_thm("arm_EOR2'",
   ``(ARM_PROG2:^(ty_antiq ARM_PROG2_type)) c_flag
            (R a x * R b y * S (sN,sZ,sC,sV) * PASS c_flag (sN,sZ,sC,sV))
-           [enc (EOR c_flag s_flag a a (ADDR_MODE1_CMD a_mode b))]
+           [enc (EOR c_flag s_flag a a (ADDR_MODE1_CMD a_mode b))] {}
            (R a (x ?? SND (ADDR_MODE1_VAL a_mode y sC)) * R b y *
             S
               ((if s_flag then
@@ -5157,7 +4814,7 @@ val arm_EOR2' = store_thm("arm_EOR2'",
 val arm_ORR2' = store_thm("arm_ORR2'",
   ``(ARM_PROG2:^(ty_antiq ARM_PROG2_type)) c_flag
            (R a x * R b y * S (sN,sZ,sC,sV) * PASS c_flag (sN,sZ,sC,sV))
-           [enc (ORR c_flag s_flag a a (ADDR_MODE1_CMD a_mode b))]
+           [enc (ORR c_flag s_flag a a (ADDR_MODE1_CMD a_mode b))] {}
            (R a (x !! SND (ADDR_MODE1_VAL a_mode y sC)) * R b y *
             S
               ((if s_flag then
@@ -5177,7 +4834,7 @@ val arm_ORR2' = store_thm("arm_ORR2'",
 val arm_RSB2' = store_thm("arm_RSB2'",
   ``(ARM_PROG2:^(ty_antiq ARM_PROG2_type)) c_flag
            (R a x * R b y * S (sN,sZ,sC,sV) * PASS c_flag (sN,sZ,sC,sV))
-           [enc (RSB c_flag s_flag a a (ADDR_MODE1_CMD a_mode b))]
+           [enc (RSB c_flag s_flag a a (ADDR_MODE1_CMD a_mode b))] {}
            (R a (SND (ADDR_MODE1_VAL a_mode y sC) - x) * R b y *
             S
               (if s_flag then
@@ -5200,7 +4857,7 @@ val arm_RSB2' = store_thm("arm_RSB2'",
 val arm_RSC2' = store_thm("arm_RSC2'",
   ``(ARM_PROG2:^(ty_antiq ARM_PROG2_type)) c_flag
            (R a x * R b y * S (sN,sZ,sC,sV) * PASS c_flag (sN,sZ,sC,sV))
-           [enc (RSC c_flag s_flag a a (ADDR_MODE1_CMD a_mode b))]
+           [enc (RSC c_flag s_flag a a (ADDR_MODE1_CMD a_mode b))] {}
            (R a (SND (ADDR_MODE1_VAL a_mode y sC) - x - (if sC then 0w else 1w)) * R b y *
             S
               (if s_flag then
@@ -5224,7 +4881,7 @@ val arm_RSC2' = store_thm("arm_RSC2'",
 val arm_SBC2' = store_thm("arm_SBC2'",
   ``(ARM_PROG2:^(ty_antiq ARM_PROG2_type)) c_flag
            (R a x * R b y * S (sN,sZ,sC,sV) * PASS c_flag (sN,sZ,sC,sV))
-           [enc (SBC c_flag s_flag a a (ADDR_MODE1_CMD a_mode b))]
+           [enc (SBC c_flag s_flag a a (ADDR_MODE1_CMD a_mode b))] {}
            (R a (x - SND (ADDR_MODE1_VAL a_mode y sC) - (if sC then 0w else 1w)) * R b y *
             S
               (if s_flag then
@@ -5248,7 +4905,7 @@ val arm_SBC2' = store_thm("arm_SBC2'",
 val arm_SUB2' = store_thm("arm_SUB2'",
   ``(ARM_PROG2:^(ty_antiq ARM_PROG2_type)) c_flag
            (R a x * R b y * S (sN,sZ,sC,sV) * PASS c_flag (sN,sZ,sC,sV))
-           [enc (SUB c_flag s_flag a a (ADDR_MODE1_CMD a_mode b))]
+           [enc (SUB c_flag s_flag a a (ADDR_MODE1_CMD a_mode b))] {}
            (R a (x - SND (ADDR_MODE1_VAL a_mode y sC)) * R b y *
             S
               (if s_flag then
@@ -5270,7 +4927,7 @@ val arm_SUB2' = store_thm("arm_SUB2'",
 val arm_ADC2'' = store_thm("arm_ADC2''",
   ``(ARM_PROG2:^(ty_antiq ARM_PROG2_type)) c_flag
            (R a x * R b y * S (sN,sZ,sC,sV) * PASS c_flag (sN,sZ,sC,sV))
-           [enc (ADC c_flag s_flag b a (ADDR_MODE1_CMD a_mode a))]
+           [enc (ADC c_flag s_flag b a (ADDR_MODE1_CMD a_mode a))] {}
            (R a x *
             R b (x + SND (ADDR_MODE1_VAL a_mode x sC) + (if sC then 1w else 0w)) *
             S
@@ -5300,7 +4957,7 @@ val arm_ADC2'' = store_thm("arm_ADC2''",
 val arm_ADD2'' = store_thm("arm_ADD2''",
   ``(ARM_PROG2:^(ty_antiq ARM_PROG2_type)) c_flag
            (R a x * R b y * S (sN,sZ,sC,sV) * PASS c_flag (sN,sZ,sC,sV))
-           [enc (ADD c_flag s_flag b a (ADDR_MODE1_CMD a_mode a))]
+           [enc (ADD c_flag s_flag b a (ADDR_MODE1_CMD a_mode a))] {}
            (R a x * R b (x + SND (ADDR_MODE1_VAL a_mode x sC)) *
             S
               (if s_flag then
@@ -5322,7 +4979,7 @@ val arm_ADD2'' = store_thm("arm_ADD2''",
 val arm_AND2'' = store_thm("arm_AND2''",
   ``(ARM_PROG2:^(ty_antiq ARM_PROG2_type)) c_flag
            (R a x * R b y * S (sN,sZ,sC,sV) * PASS c_flag (sN,sZ,sC,sV))
-           [enc (AND c_flag s_flag b a (ADDR_MODE1_CMD a_mode a))]
+           [enc (AND c_flag s_flag b a (ADDR_MODE1_CMD a_mode a))] {}
            (R a x * R b (x && SND (ADDR_MODE1_VAL a_mode x sC)) *
             S
               ((if s_flag then
@@ -5342,7 +4999,7 @@ val arm_AND2'' = store_thm("arm_AND2''",
 val arm_BIC2'' = store_thm("arm_BIC2''",
   ``(ARM_PROG2:^(ty_antiq ARM_PROG2_type)) c_flag
            (R a x * R b y * S (sN,sZ,sC,sV) * PASS c_flag (sN,sZ,sC,sV))
-           [enc (BIC c_flag s_flag b a (ADDR_MODE1_CMD a_mode a))]
+           [enc (BIC c_flag s_flag b a (ADDR_MODE1_CMD a_mode a))] {}
            (R a x * R b (x && ~SND (ADDR_MODE1_VAL a_mode x sC)) *
             S
               ((if s_flag then
@@ -5362,7 +5019,7 @@ val arm_BIC2'' = store_thm("arm_BIC2''",
 val arm_EOR2'' = store_thm("arm_EOR2''",
   ``(ARM_PROG2:^(ty_antiq ARM_PROG2_type)) c_flag
            (R a x * R b y * S (sN,sZ,sC,sV) * PASS c_flag (sN,sZ,sC,sV))
-           [enc (EOR c_flag s_flag b a (ADDR_MODE1_CMD a_mode a))]
+           [enc (EOR c_flag s_flag b a (ADDR_MODE1_CMD a_mode a))] {}
            (R a x * R b (x ?? SND (ADDR_MODE1_VAL a_mode x sC)) *
             S
               ((if s_flag then
@@ -5382,7 +5039,7 @@ val arm_EOR2'' = store_thm("arm_EOR2''",
 val arm_ORR2'' = store_thm("arm_ORR2''",
   ``(ARM_PROG2:^(ty_antiq ARM_PROG2_type)) c_flag
            (R a x * R b y * S (sN,sZ,sC,sV) * PASS c_flag (sN,sZ,sC,sV))
-           [enc (ORR c_flag s_flag b a (ADDR_MODE1_CMD a_mode a))]
+           [enc (ORR c_flag s_flag b a (ADDR_MODE1_CMD a_mode a))] {}
            (R a x * R b (x !! SND (ADDR_MODE1_VAL a_mode x sC)) *
             S
               ((if s_flag then
@@ -5402,7 +5059,7 @@ val arm_ORR2'' = store_thm("arm_ORR2''",
 val arm_RSB2'' = store_thm("arm_RSB2''",
   ``(ARM_PROG2:^(ty_antiq ARM_PROG2_type)) c_flag
            (R a x * R b y * S (sN,sZ,sC,sV) * PASS c_flag (sN,sZ,sC,sV))
-           [enc (RSB c_flag s_flag b a (ADDR_MODE1_CMD a_mode a))]
+           [enc (RSB c_flag s_flag b a (ADDR_MODE1_CMD a_mode a))] {}
            (R a x * R b (SND (ADDR_MODE1_VAL a_mode x sC) - x) *
             S
               (if s_flag then
@@ -5425,7 +5082,7 @@ val arm_RSB2'' = store_thm("arm_RSB2''",
 val arm_RSC2'' = store_thm("arm_RSC2''",
   ``(ARM_PROG2:^(ty_antiq ARM_PROG2_type)) c_flag
            (R a x * R b y * S (sN,sZ,sC,sV) * PASS c_flag (sN,sZ,sC,sV))
-           [enc (RSC c_flag s_flag b a (ADDR_MODE1_CMD a_mode a))]
+           [enc (RSC c_flag s_flag b a (ADDR_MODE1_CMD a_mode a))] {}
            (R a x *
             R b (SND (ADDR_MODE1_VAL a_mode x sC) - x - (if sC then 0w else 1w)) *
             S
@@ -5450,7 +5107,7 @@ val arm_RSC2'' = store_thm("arm_RSC2''",
 val arm_SBC2'' = store_thm("arm_SBC2''",
   ``(ARM_PROG2:^(ty_antiq ARM_PROG2_type)) c_flag
            (R a x * R b y * S (sN,sZ,sC,sV) * PASS c_flag (sN,sZ,sC,sV))
-           [enc (SBC c_flag s_flag b a (ADDR_MODE1_CMD a_mode a))]
+           [enc (SBC c_flag s_flag b a (ADDR_MODE1_CMD a_mode a))] {}
            (R a x * R b (x - SND (ADDR_MODE1_VAL a_mode x sC) - (if sC then 0w else 1w)) *
             S
               (if s_flag then
@@ -5474,7 +5131,7 @@ val arm_SBC2'' = store_thm("arm_SBC2''",
 val arm_SUB2'' = store_thm("arm_SUB2''",
   ``(ARM_PROG2:^(ty_antiq ARM_PROG2_type)) c_flag
            (R a x * R b y * S (sN,sZ,sC,sV) * PASS c_flag (sN,sZ,sC,sV))
-           [enc (SUB c_flag s_flag b a (ADDR_MODE1_CMD a_mode a))]
+           [enc (SUB c_flag s_flag b a (ADDR_MODE1_CMD a_mode a))] {}
            (R a x * R b (x - SND (ADDR_MODE1_VAL a_mode x sC)) *
             S
               (if s_flag then
@@ -5496,7 +5153,7 @@ val arm_SUB2'' = store_thm("arm_SUB2''",
 val arm_ADC3 = store_thm("arm_ADC3",
   ``(ARM_PROG2:^(ty_antiq ARM_PROG2_type)) c_flag
            (R a x * R b y * R c z * S (sN,sZ,sC,sV) * PASS c_flag (sN,sZ,sC,sV))
-           [enc (ADC c_flag s_flag c a (ADDR_MODE1_CMD a_mode b))]
+           [enc (ADC c_flag s_flag c a (ADDR_MODE1_CMD a_mode b))] {}
            (R a x * R b y *
             R c (x + SND (ADDR_MODE1_VAL a_mode y sC) + (if sC then 1w else 0w)) *
             S
@@ -5526,7 +5183,7 @@ val arm_ADC3 = store_thm("arm_ADC3",
 val arm_ADD3 = store_thm("arm_ADD3",
   ``(ARM_PROG2:^(ty_antiq ARM_PROG2_type)) c_flag
            (R a x * R b y * R c z * S (sN,sZ,sC,sV) * PASS c_flag (sN,sZ,sC,sV))
-           [enc (ADD c_flag s_flag c a (ADDR_MODE1_CMD a_mode b))]
+           [enc (ADD c_flag s_flag c a (ADDR_MODE1_CMD a_mode b))] {}
            (R a x * R b y * R c (x + SND (ADDR_MODE1_VAL a_mode y sC)) *
             S
               (if s_flag then
@@ -5548,7 +5205,7 @@ val arm_ADD3 = store_thm("arm_ADD3",
 val arm_AND3 = store_thm("arm_AND3",
   ``(ARM_PROG2:^(ty_antiq ARM_PROG2_type)) c_flag
            (R a x * R b y * R c z * S (sN,sZ,sC,sV) * PASS c_flag (sN,sZ,sC,sV))
-           [enc (AND c_flag s_flag c a (ADDR_MODE1_CMD a_mode b))]
+           [enc (AND c_flag s_flag c a (ADDR_MODE1_CMD a_mode b))] {}
            (R a x * R b y * R c (x && SND (ADDR_MODE1_VAL a_mode y sC)) *
             S
               ((if s_flag then
@@ -5568,7 +5225,7 @@ val arm_AND3 = store_thm("arm_AND3",
 val arm_BIC3 = store_thm("arm_BIC3",
   ``(ARM_PROG2:^(ty_antiq ARM_PROG2_type)) c_flag
            (R a x * R b y * R c z * S (sN,sZ,sC,sV) * PASS c_flag (sN,sZ,sC,sV))
-           [enc (BIC c_flag s_flag c a (ADDR_MODE1_CMD a_mode b))]
+           [enc (BIC c_flag s_flag c a (ADDR_MODE1_CMD a_mode b))] {}
            (R a x * R b y * R c (x && ~SND (ADDR_MODE1_VAL a_mode y sC)) *
             S
               ((if s_flag then
@@ -5588,7 +5245,7 @@ val arm_BIC3 = store_thm("arm_BIC3",
 val arm_EOR3 = store_thm("arm_EOR3",
   ``(ARM_PROG2:^(ty_antiq ARM_PROG2_type)) c_flag
            (R a x * R b y * R c z * S (sN,sZ,sC,sV) * PASS c_flag (sN,sZ,sC,sV))
-           [enc (EOR c_flag s_flag c a (ADDR_MODE1_CMD a_mode b))]
+           [enc (EOR c_flag s_flag c a (ADDR_MODE1_CMD a_mode b))] {}
            (R a x * R b y * R c (x ?? SND (ADDR_MODE1_VAL a_mode y sC)) *
             S
               ((if s_flag then
@@ -5608,7 +5265,7 @@ val arm_EOR3 = store_thm("arm_EOR3",
 val arm_ORR3 = store_thm("arm_ORR3",
   ``(ARM_PROG2:^(ty_antiq ARM_PROG2_type)) c_flag
            (R a x * R b y * R c z * S (sN,sZ,sC,sV) * PASS c_flag (sN,sZ,sC,sV))
-           [enc (ORR c_flag s_flag c a (ADDR_MODE1_CMD a_mode b))]
+           [enc (ORR c_flag s_flag c a (ADDR_MODE1_CMD a_mode b))] {}
            (R a x * R b y * R c (x !! SND (ADDR_MODE1_VAL a_mode y sC)) *
             S
               ((if s_flag then
@@ -5628,7 +5285,7 @@ val arm_ORR3 = store_thm("arm_ORR3",
 val arm_RSB3 = store_thm("arm_RSB3",
   ``(ARM_PROG2:^(ty_antiq ARM_PROG2_type)) c_flag
            (R a x * R b y * R c z * S (sN,sZ,sC,sV) * PASS c_flag (sN,sZ,sC,sV))
-           [enc (RSB c_flag s_flag c a (ADDR_MODE1_CMD a_mode b))]
+           [enc (RSB c_flag s_flag c a (ADDR_MODE1_CMD a_mode b))] {}
            (R a x * R b y * R c (SND (ADDR_MODE1_VAL a_mode y sC) - x) *
             S
               (if s_flag then
@@ -5651,7 +5308,7 @@ val arm_RSB3 = store_thm("arm_RSB3",
 val arm_RSC3 = store_thm("arm_RSC3",
   ``(ARM_PROG2:^(ty_antiq ARM_PROG2_type)) c_flag
            (R a x * R b y * R c z * S (sN,sZ,sC,sV) * PASS c_flag (sN,sZ,sC,sV))
-           [enc (RSC c_flag s_flag c a (ADDR_MODE1_CMD a_mode b))]
+           [enc (RSC c_flag s_flag c a (ADDR_MODE1_CMD a_mode b))] {}
            (R a x * R b y *
             R c (SND (ADDR_MODE1_VAL a_mode y sC) - x - (if sC then 0w else 1w)) *
             S
@@ -5676,7 +5333,7 @@ val arm_RSC3 = store_thm("arm_RSC3",
 val arm_SBC3 = store_thm("arm_SBC3",
   ``(ARM_PROG2:^(ty_antiq ARM_PROG2_type)) c_flag
            (R a x * R b y * R c z * S (sN,sZ,sC,sV) * PASS c_flag (sN,sZ,sC,sV))
-           [enc (SBC c_flag s_flag c a (ADDR_MODE1_CMD a_mode b))]
+           [enc (SBC c_flag s_flag c a (ADDR_MODE1_CMD a_mode b))] {}
            (R a x * R b y * R c (x - SND (ADDR_MODE1_VAL a_mode y sC) - (if sC then 0w else 1w)) *
             S
               (if s_flag then
@@ -5700,7 +5357,7 @@ val arm_SBC3 = store_thm("arm_SBC3",
 val arm_SUB3 = store_thm("arm_SUB3",
   ``(ARM_PROG2:^(ty_antiq ARM_PROG2_type)) c_flag
            (R a x * R b y * R c z * S (sN,sZ,sC,sV) * PASS c_flag (sN,sZ,sC,sV))
-           [enc (SUB c_flag s_flag c a (ADDR_MODE1_CMD a_mode b))]
+           [enc (SUB c_flag s_flag c a (ADDR_MODE1_CMD a_mode b))] {}
            (R a x * R b y * R c (x - SND (ADDR_MODE1_VAL a_mode y sC)) *
             S
               (if s_flag then
@@ -5826,7 +5483,7 @@ val arm_B = store_thm("arm_B",
 val arm_B2 = store_thm("arm_B2",
   ``(ARM_PROG2:^(ty_antiq ARM_PROG2_type)) c_flag 
            (S (sN,sZ,sC,sV) * PASS c_flag (sN,sZ,sC,sV)) 
-           [enc (B c_flag offset)] SEP_F        
+           [enc (B c_flag offset)] {} SEP_F        
            {(S (sN,sZ,sC,sV),pcADD (sw2sw offset + 2w))}``,
   ARM_PROG2_INIT_TAC ARM_B_NOP
       `st*cd*cmd*pc*ud` `pc*cmd*st*ud*cd`
@@ -5842,7 +5499,7 @@ val arm_MOV_PC_GENERAL = store_thm("arm_MOV_PC_GENERAL",
   ``(ARM_PROG2:^(ty_antiq ARM_PROG2_type)) c_flag
            (R a x * S (sN,sZ,sC,sV) * PASS c_flag (sN,sZ,sC,sV) * 
             cond (SND (ADDR_MODE1_VAL a_mode x sC) && 3w = 0w))
-           [enc (MOV c_flag F 15w (ADDR_MODE1_CMD a_mode a))] SEP_F
+           [enc (MOV c_flag F 15w (ADDR_MODE1_CMD a_mode a))] {} SEP_F
            {(~R a * S (sN,sZ,sC,sV),pcSET (addr30 (SND (ADDR_MODE1_VAL a_mode x sC))))}``,
   REWRITE_TAC [R30_def]
   \\ ARM_PROG2_INIT_TAC ARM_MOV_NOP
@@ -5865,7 +5522,7 @@ val arm_MOV_PC_PRECISE = store_thm("arm_MOV_PC_PRECISE",
   ``(ARM_PROG2:^(ty_antiq ARM_PROG2_type)) c_flag
            (R a x * S (sN,sZ,sC,sV) * PASS c_flag (sN,sZ,sC,sV) * 
             cond (SND (ADDR_MODE1_VAL a_mode x sC) && 3w = 0w))
-           [enc (MOV c_flag F 15w (ADDR_MODE1_CMD a_mode a))] SEP_F
+           [enc (MOV c_flag F 15w (ADDR_MODE1_CMD a_mode a))] {} SEP_F
            {(R a x * S (sN,sZ,sC,sV),pcSET (addr30 (SND (ADDR_MODE1_VAL a_mode x sC))))}``,
   REWRITE_TAC [R30_def]
   \\ ARM_PROG2_INIT_TAC ARM_MOV_NOP
@@ -5883,21 +5540,6 @@ val arm_MOV_PC_PRECISE = store_thm("arm_MOV_PC_PRECISE",
 val arm_blal_pre = sep_pred_semantics (xR2',xMm,`(F,st)`,`(T,ud)`,`(F,rt)`,`(F,g)`);
 val arm_blal_post = sep_pred_semantics (xR2,xMm,`(F,st)`,`(T,ud)`,`(F,rt)`,`(F,g)`);
 
-(*
-
-  ``ARM_RUN (R 14w x * ARMpc (addr30 p) * mpool ARMi (addr30 p) {([enc (BL AL offset)],I)})
-            (R 14w (p + 4w) * ARMpc (addr30 p + sw2sw offset + 2w) * 
-             mpool ARMi (addr30 p) {([enc (BL AL offset)],I)})``   
-  REWRITE_TAC [GSYM ARMproc_def,GSYM ARM_RUN_def,ARMpc_def,STAR_ASSOC,ARM_RUN_SEMANTICS]
-  \\ REPEAT STRIP_TAC \\ Q.EXISTS_TAC `1` 
-  \\ FULL_SIMP_TAC (std_ss++sep_ss) [LET_DEF,STATE_ARM_MEM_1,ARMpc_def,R30_def,pcINC_def, 
-       SIMP_RULE std_ss [LENGTH] (Q.SPEC `[cmd]` mpool_eq_ms),ms_def,STAR_ASSOC,
-       wLENGTH_def,LENGTH,GSYM PC_SIMP]
-  \\ FULL_MOVE_STAR_TAC `a*pc*ud*m` `a*pc*m*ud`  
-  \\ FULL_SIMP_TAC bool_ss [arm_blal_pre,arm_blal_post]
-
-  *)
-
 val WORD_LSL_EQ_MULT = prove(
   ``!x. x << n = x * n2w (2 ** n)``,
   Cases_word \\ REWRITE_TAC [word_lsl_n2w,word_mul_n2w]
@@ -5913,7 +5555,7 @@ val arm_bl_post = sep_pred_semantics (xR2,xMm,`(T,st)`,`(T,ud)`,`(F,rt)`,`(T,g)`
 
 val ARM_SPEC_BL = prove(
   ``ARM_SPEC2 c (R 14w x * PASS c (sN,sZ,sC,sV) * S (sN,sZ,sC,sV),p) 
-                [enc (BL c offset)] 
+                {([enc (BL c offset)],p)} 
                 (R 14w (p + 4w) * S (sN,sZ,sC,sV),p + 8w + sw2sw offset * 4w)``,
   REWRITE_TAC [ARM_SPEC2_def] \\ ONCE_REWRITE_TAC [CONJ_COMM] \\ REPEAT STRIP_TAC
   THEN1 (Q.SPEC_TAC (`p`,`p`) \\ MATCH_MP_TAC SPEC_ARM_MODEL_INTRO
